@prefix dcterms: <http://purl.org/dc/terms/> .
@prefix emmo: <http://emmo.info/domains/emmo-material.owl#> .
@prefix mdo-core: <https://w3id.org/mdo/core/> .
@prefix ns1: <https://qudt.org/schema/qudt/> .
@prefix ns2: <https://qudt.org/schema/qudt#> .
@prefix ns3: <https://github.com/DeperiasKerre/qcl_Onto/blob/main/qclontology/version-1.0/qclonto.owl#> .
@prefix owl: <http://www.w3.org/2002/07/owl#> .
@prefix prov: <http://www.w3.org/ns/prov#> .
@prefix rdf: <http://www.w3.org/1999/02/22-rdf-syntax-ns#> .
@prefix rdfs: <http://www.w3.org/2000/01/rdf-schema#> .
@prefix vann: <http://purl.org/vocab/vann/> .
@prefix xsd: <http://www.w3.org/2001/XMLSchema#> .

<('https://github.com/DeperiasKerre/qcl_Onto/blob/main/qclontology/version-1.0/qclonto.owl#f1',)> a ns3:LasingFrequency .

<('https://github.com/DeperiasKerre/qcl_Onto/blob/main/qclontology/version-1.0/qclonto.owl#f10',)> a ns3:FrequencyValue,
        ns3:LasingFrequency .

<('https://github.com/DeperiasKerre/qcl_Onto/blob/main/qclontology/version-1.0/qclonto.owl#f11',)> a ns3:FrequencyValue,
        ns3:LasingFrequency .

<('https://github.com/DeperiasKerre/qcl_Onto/blob/main/qclontology/version-1.0/qclonto.owl#f12',)> a ns3:FrequencyValue,
        ns3:LasingFrequency .

<('https://github.com/DeperiasKerre/qcl_Onto/blob/main/qclontology/version-1.0/qclonto.owl#f13',)> a ns3:FrequencyValue,
        ns3:LasingFrequency .

<('https://github.com/DeperiasKerre/qcl_Onto/blob/main/qclontology/version-1.0/qclonto.owl#f2',)> a ns3:LasingFrequency .

<('https://github.com/DeperiasKerre/qcl_Onto/blob/main/qclontology/version-1.0/qclonto.owl#f3',)> a ns3:LasingFrequency .

<('https://github.com/DeperiasKerre/qcl_Onto/blob/main/qclontology/version-1.0/qclonto.owl#f4',)> a ns3:LasingFrequency .

<('https://github.com/DeperiasKerre/qcl_Onto/blob/main/qclontology/version-1.0/qclonto.owl#f5',)> a ns3:LasingFrequency .

<('https://github.com/DeperiasKerre/qcl_Onto/blob/main/qclontology/version-1.0/qclonto.owl#f6',)> a ns3:LasingFrequency .

<('https://github.com/DeperiasKerre/qcl_Onto/blob/main/qclontology/version-1.0/qclonto.owl#f7',)> a ns3:LasingFrequency .

<('https://github.com/DeperiasKerre/qcl_Onto/blob/main/qclontology/version-1.0/qclonto.owl#f8',)> a ns3:LasingFrequency .

<('https://github.com/DeperiasKerre/qcl_Onto/blob/main/qclontology/version-1.0/qclonto.owl#f9',)> a ns3:LasingFrequency .

<('https://github.com/DeperiasKerre/qcl_Onto/blob/main/qclontology/version-1.0/qclonto.owl#fv1',)> a ns3:FrequencyValue .

<('https://github.com/DeperiasKerre/qcl_Onto/blob/main/qclontology/version-1.0/qclonto.owl#fv2',)> a ns3:FrequencyValue .

<('https://github.com/DeperiasKerre/qcl_Onto/blob/main/qclontology/version-1.0/qclonto.owl#fv3',)> a ns3:FrequencyValue .

<('https://github.com/DeperiasKerre/qcl_Onto/blob/main/qclontology/version-1.0/qclonto.owl#fv4',)> a ns3:FrequencyValue .

<('https://github.com/DeperiasKerre/qcl_Onto/blob/main/qclontology/version-1.0/qclonto.owl#fv5',)> a ns3:FrequencyValue .

<('https://github.com/DeperiasKerre/qcl_Onto/blob/main/qclontology/version-1.0/qclonto.owl#fv6',)> a ns3:FrequencyValue .

<('https://github.com/DeperiasKerre/qcl_Onto/blob/main/qclontology/version-1.0/qclonto.owl#fv7',)> a ns3:FrequencyValue .

<('https://github.com/DeperiasKerre/qcl_Onto/blob/main/qclontology/version-1.0/qclonto.owl#fv8',)> a ns3:FrequencyValue .

<('https://github.com/DeperiasKerre/qcl_Onto/blob/main/qclontology/version-1.0/qclonto.owl#fv9',)> a ns3:FrequencyValue .

<('https://github.com/DeperiasKerre/qcl_Onto/blob/main/qclontology/version-1.0/qclonto.owl#p1',)> a ns3:OpticalPower .

<('https://github.com/DeperiasKerre/qcl_Onto/blob/main/qclontology/version-1.0/qclonto.owl#p2',)> a ns3:OpticalPower .

<('https://github.com/DeperiasKerre/qcl_Onto/blob/main/qclontology/version-1.0/qclonto.owl#p3',)> a ns3:OpticalPower .

<('https://github.com/DeperiasKerre/qcl_Onto/blob/main/qclontology/version-1.0/qclonto.owl#p4',)> a ns3:OpticalPower .

<('https://github.com/DeperiasKerre/qcl_Onto/blob/main/qclontology/version-1.0/qclonto.owl#p5',)> a ns3:OpticalPower .

<('https://github.com/DeperiasKerre/qcl_Onto/blob/main/qclontology/version-1.0/qclonto.owl#p6',)> a ns3:OpticalPower .

<('https://github.com/DeperiasKerre/qcl_Onto/blob/main/qclontology/version-1.0/qclonto.owl#p7',)> a ns3:OpticalPower .

<('https://github.com/DeperiasKerre/qcl_Onto/blob/main/qclontology/version-1.0/qclonto.owl#p8',)> a ns3:OpticalPower .

<('https://github.com/DeperiasKerre/qcl_Onto/blob/main/qclontology/version-1.0/qclonto.owl#p9',)> a ns3:OpticalPower .

<('https://github.com/DeperiasKerre/qcl_Onto/blob/main/qclontology/version-1.0/qclonto.owl#pv1',)> a ns3:PowerValue .

<('https://github.com/DeperiasKerre/qcl_Onto/blob/main/qclontology/version-1.0/qclonto.owl#pv2',)> a ns3:PowerValue .

<('https://github.com/DeperiasKerre/qcl_Onto/blob/main/qclontology/version-1.0/qclonto.owl#pv3',)> a ns3:PowerValue .

<('https://github.com/DeperiasKerre/qcl_Onto/blob/main/qclontology/version-1.0/qclonto.owl#pv4',)> a ns3:PowerValue .

<('https://github.com/DeperiasKerre/qcl_Onto/blob/main/qclontology/version-1.0/qclonto.owl#pv5',)> a ns3:PowerValue .

<('https://github.com/DeperiasKerre/qcl_Onto/blob/main/qclontology/version-1.0/qclonto.owl#pv6',)> a ns3:PowerValue .

<('https://github.com/DeperiasKerre/qcl_Onto/blob/main/qclontology/version-1.0/qclonto.owl#pv7',)> a ns3:PowerValue .

<('https://github.com/DeperiasKerre/qcl_Onto/blob/main/qclontology/version-1.0/qclonto.owl#pv8',)> a ns3:PowerValue .

<('https://github.com/DeperiasKerre/qcl_Onto/blob/main/qclontology/version-1.0/qclonto.owl#pv9',)> a ns3:PowerValue .

<('https://github.com/DeperiasKerre/qcl_Onto/blob/main/qclontology/version-1.0/qclonto.owl#tp1',)> a ns3:WorkingTemperature .

<('https://github.com/DeperiasKerre/qcl_Onto/blob/main/qclontology/version-1.0/qclonto.owl#tp10',)> a ns3:WorkingTemperature .

<('https://github.com/DeperiasKerre/qcl_Onto/blob/main/qclontology/version-1.0/qclonto.owl#tp11',)> a ns3:WorkingTemperature .

<('https://github.com/DeperiasKerre/qcl_Onto/blob/main/qclontology/version-1.0/qclonto.owl#tp12',)> a ns3:WorkingTemperature .

<('https://github.com/DeperiasKerre/qcl_Onto/blob/main/qclontology/version-1.0/qclonto.owl#tp13',)> a ns3:WorkingTemperature .

<('https://github.com/DeperiasKerre/qcl_Onto/blob/main/qclontology/version-1.0/qclonto.owl#tp14',)> a ns3:WorkingTemperature .

<('https://github.com/DeperiasKerre/qcl_Onto/blob/main/qclontology/version-1.0/qclonto.owl#tp15',)> a ns3:WorkingTemperature .

<('https://github.com/DeperiasKerre/qcl_Onto/blob/main/qclontology/version-1.0/qclonto.owl#tp16',)> a ns3:WorkingTemperature .

<('https://github.com/DeperiasKerre/qcl_Onto/blob/main/qclontology/version-1.0/qclonto.owl#tp17',)> a ns3:WorkingTemperature .

<('https://github.com/DeperiasKerre/qcl_Onto/blob/main/qclontology/version-1.0/qclonto.owl#tp18',)> a ns3:WorkingTemperature .

<('https://github.com/DeperiasKerre/qcl_Onto/blob/main/qclontology/version-1.0/qclonto.owl#tp2',)> a ns3:WorkingTemperature .

<('https://github.com/DeperiasKerre/qcl_Onto/blob/main/qclontology/version-1.0/qclonto.owl#tp3',)> a ns3:WorkingTemperature .

<('https://github.com/DeperiasKerre/qcl_Onto/blob/main/qclontology/version-1.0/qclonto.owl#tp4',)> a ns3:WorkingTemperature .

<('https://github.com/DeperiasKerre/qcl_Onto/blob/main/qclontology/version-1.0/qclonto.owl#tp5',)> a ns3:WorkingTemperature .

<('https://github.com/DeperiasKerre/qcl_Onto/blob/main/qclontology/version-1.0/qclonto.owl#tp6',)> a ns3:WorkingTemperature .

<('https://github.com/DeperiasKerre/qcl_Onto/blob/main/qclontology/version-1.0/qclonto.owl#tp7',)> a ns3:WorkingTemperature .

<('https://github.com/DeperiasKerre/qcl_Onto/blob/main/qclontology/version-1.0/qclonto.owl#tp8',)> a ns3:WorkingTemperature .

<('https://github.com/DeperiasKerre/qcl_Onto/blob/main/qclontology/version-1.0/qclonto.owl#tp9',)> a ns3:WorkingTemperature .

<('https://github.com/DeperiasKerre/qcl_Onto/blob/main/qclontology/version-1.0/qclonto.owl#tv1',)> a ns3:WorkingTempValue .

<('https://github.com/DeperiasKerre/qcl_Onto/blob/main/qclontology/version-1.0/qclonto.owl#tv10',)> a ns3:WorkingTempValue .

<('https://github.com/DeperiasKerre/qcl_Onto/blob/main/qclontology/version-1.0/qclonto.owl#tv11',)> a ns3:WorkingTempValue .

<('https://github.com/DeperiasKerre/qcl_Onto/blob/main/qclontology/version-1.0/qclonto.owl#tv12',)> a ns3:WorkingTempValue .

<('https://github.com/DeperiasKerre/qcl_Onto/blob/main/qclontology/version-1.0/qclonto.owl#tv13',)> a ns3:WorkingTempValue .

<('https://github.com/DeperiasKerre/qcl_Onto/blob/main/qclontology/version-1.0/qclonto.owl#tv14',)> a ns3:WorkingTempValue .

<('https://github.com/DeperiasKerre/qcl_Onto/blob/main/qclontology/version-1.0/qclonto.owl#tv15',)> a ns3:WorkingTempValue .

<('https://github.com/DeperiasKerre/qcl_Onto/blob/main/qclontology/version-1.0/qclonto.owl#tv16',)> a ns3:WorkingTempValue .

<('https://github.com/DeperiasKerre/qcl_Onto/blob/main/qclontology/version-1.0/qclonto.owl#tv17',)> a ns3:WorkingTempValue .

<('https://github.com/DeperiasKerre/qcl_Onto/blob/main/qclontology/version-1.0/qclonto.owl#tv18',)> a ns3:WorkingTempValue .

<('https://github.com/DeperiasKerre/qcl_Onto/blob/main/qclontology/version-1.0/qclonto.owl#tv2',)> a ns3:WorkingTempValue .

<('https://github.com/DeperiasKerre/qcl_Onto/blob/main/qclontology/version-1.0/qclonto.owl#tv3',)> a ns3:WorkingTempValue .

<('https://github.com/DeperiasKerre/qcl_Onto/blob/main/qclontology/version-1.0/qclonto.owl#tv4',)> a ns3:WorkingTempValue .

<('https://github.com/DeperiasKerre/qcl_Onto/blob/main/qclontology/version-1.0/qclonto.owl#tv5',)> a ns3:WorkingTempValue .

<('https://github.com/DeperiasKerre/qcl_Onto/blob/main/qclontology/version-1.0/qclonto.owl#tv6',)> a ns3:WorkingTempValue .

<('https://github.com/DeperiasKerre/qcl_Onto/blob/main/qclontology/version-1.0/qclonto.owl#tv7',)> a ns3:WorkingTempValue .

<('https://github.com/DeperiasKerre/qcl_Onto/blob/main/qclontology/version-1.0/qclonto.owl#tv8',)> a ns3:WorkingTempValue .

<('https://github.com/DeperiasKerre/qcl_Onto/blob/main/qclontology/version-1.0/qclonto.owl#tv9',)> a ns3:WorkingTempValue .

<(rdflib.term.URIRef('https://qudt.org/vocab/unit/K'),)> a ns1:Unit .

<(rdflib.term.URIRef('https://qudt.org/vocab/unit/MilliW'),)> a ns1:Unit .

<(rdflib.term.URIRef('https://qudt.org/vocab/unit/TeraHZ'),)> a ns1:Unit .

dcterms:contributor a owl:AnnotationProperty .

dcterms:created a owl:AnnotationProperty .

dcterms:creator a owl:AnnotationProperty .

dcterms:license a owl:AnnotationProperty .

dcterms:title a owl:AnnotationProperty .

vann:preferredNamespacePrefix a owl:AnnotationProperty .

vann:preferredNamespaceUri a owl:AnnotationProperty .

<http://qudt.org/schema/qudt/hasUnit> a owl:ObjectProperty ;
    rdfs:label "has unit"@en ;
    rdfs:comment "hasUnit represents that a quantity value has a unit."@en ;
    rdfs:domain ns3:LayerSequence,
        ns1:QuantityValue .

prov:wasAttributedTo a owl:ObjectProperty ;
    rdfs:comment "wasAttributedTo represents the relationship  quantum cascade laser device and the scientific article documenting its design and performance properties."@en ;
    rdfs:domain ns3:QuantumCascadeLaser .

ns3: a owl:Ontology ;
    dcterms:contributor "Anne Laurent",
        "Dicskson Owuor",
        "Kenneth Maussang" ;
    dcterms:created "2023-10-16" ;
    dcterms:creator "Deperias Kerre" ;
    dcterms:license "https://github.com/DeperiasKerre/qcl_Onto/blob/main/LICENSE" ;
    dcterms:title "An Ontology of Properties in the Quantum Cascade Laser Domain"@en ;
    vann:preferredNamespacePrefix "QpOnto"@en ;
    vann:preferredNamespaceUri "https://github.com/DeperiasKerre/qcl_Onto/blob/main/qclontology/version-1.0/qclonto.owl#"@en ;
    rdfs:comment "This is an ontological representation of properties in the quantum cascade laser domain."@en ;
    rdfs:seeAlso "https://github.com/DeperiasKerre/qcl_Onto" ;
    owl:versionIRI <https://github.com/DeperiasKerre/qcl_Onto/tree/main/qclontology/version-1.0> ;
    owl:versionInfo "1.0" .

ns3:AuthorName a owl:DatatypeProperty ;
    rdfs:comment "AuthorName represents that an academic article has the author name in a string."@en ;
    rdfs:domain <http://purl.org/ontology/bibo/AcademicArticle> ;
    rdfs:range xsd:string .

ns3:DOI a owl:DatatypeProperty ;
    rdfs:comment "DOI represents that an academic article has the DOI in a string."@en ;
    rdfs:domain <http://purl.org/ontology/bibo/AcademicArticle> ;
    rdfs:range xsd:string .

ns3:LS13 a ns3:LayerSequence ;
    ns3:sequence "3.9/14.0/ 0.6/ 9.1/ 0.6/16.0/ 1.5/12.8/ 1.8/12.2/2.0/12.0/ 2.0/ 11.4/ 2.7/11.3/ 3.5/ 11.6" .

ns3:LS15 a ns3:LayerSequence ;
    ns3:sequence "32.6/79.9/19.0/84.0/29.0/51.6" .

ns3:M13 a ns3:HeterostructureMaterials ;
    ns3:matFormula "GaAs/Al0.15Ga0.85As" .

ns3:M15 a ns3:HeterostructureMaterials ;
    ns3:matFormula "GaAs/Al0.25Ga0.75As" .

ns3:PublicationTitle a owl:DatatypeProperty ;
    rdfs:comment "PublicationTitle represents that an academic article has the publication title in a string."@en ;
    rdfs:domain <http://purl.org/ontology/bibo/AcademicArticle> ;
    rdfs:range xsd:string .

ns3:PublicationYear a owl:DatatypeProperty ;
    rdfs:comment "PublicationYear represents that an academic article has the year of publication in a an integer."@en ;
    rdfs:domain <http://purl.org/ontology/bibo/AcademicArticle> ;
    rdfs:range xsd:integer .

ns3:PublisherName a owl:DatatypeProperty ;
    rdfs:comment "PublisherName represents that an academic article has the publishers name in a string."@en ;
    rdfs:domain <http://purl.org/ontology/bibo/AcademicArticle> ;
    rdfs:range xsd:string .

ns3:QCL1 a ns3:QuantumCascadeLaser ;
    prov:wasAttributedTo <https://www.doi.org/10.1063/1.2189671> ;
    ns3:hasHeterostructure ns3:HS1 ;
    ns3:hasProperty ns3:f1,
        ns3:tp1,
        ns3:tp14 ;
    ns3:hasWorkingMode ns3:ContinousWaveOperation,
        ns3:PulsedOperation .

ns3:QCL10 a ns3:QuantumCascadeLaser ;
    prov:wasAttributedTo <https://www.doi.org/10.1088/1367-2630/17/2/023050> ;
    ns3:hasHeterostructure ns3:HS10 ;
    ns3:hasProperty ns3:tp8 ;
    ns3:hasWorkingMode ns3:ContinousWaveOperation .

ns3:QCL11 a ns3:QuantumCascadeLaser ;
    prov:wasAttributedTo <https://www.doi.org/10.1364/OE.20.003866> ;
    ns3:hasHeterostructure ns3:HS11 ;
    ns3:hasProperty ns3:f10,
        ns3:p7,
        ns3:tp9 ;
    ns3:hasWorkingMode ns3:ContinousWaveOperation .

ns3:QCL12 a ns3:QuantumCascadeLaser ;
    prov:wasAttributedTo <https://www.doi.org/10.1364/OE.16.003242> ;
    ns3:hasHeterostructure ns3:HS12 ;
    ns3:hasProperty ns3:f11,
        ns3:tp10 ;
    ns3:hasWorkingMode ns3:ContinousWaveOperation .

ns3:QCL13 a ns3:QuantumCascadeLaser ;
    prov:wasAttributedTo <https://www.doi.org/10.1063/1.2737129> ;
    ns3:hasHeterostructure ns3:HS13 ;
    ns3:hasProperty ns3:f12,
        ns3:p8,
        ns3:tp11 ;
    ns3:hasWorkingMode ns3:ContinousWaveOperation .

ns3:QCL14 a ns3:QuantumCascadeLaser ;
    prov:wasAttributedTo <https://www.doi.org/10.1063/1.2216112> ;
    ns3:hasHeterostructure ns3:HS14 ;
    ns3:hasProperty ns3:tp12,
        ns3:tp18 ;
    ns3:hasWorkingMode ns3:ContinousWaveOperation,
        ns3:PulsedOperation .

ns3:QCL15 a ns3:QuantumCascadeLaser ;
    prov:wasAttributedTo <https://www.doi.org/10.1063/1.5110305> ;
    ns3:hasHeterostructure ns3:HS15 ;
    ns3:hasProperty ns3:f13,
        ns3:p9,
        ns3:tp13 ;
    ns3:hasWorkingMode ns3:ContinousWaveOperation .

ns3:QCL2 a ns3:QuantumCascadeLaser ;
    prov:wasAttributedTo <https://opg.optica.org/oe/fulltext.cfm?uri=oe-23-15-19689&id=323020> ;
    ns3:hasHeterostructure ns3:HS2 ;
    ns3:hasProperty ns3:f2,
        ns3:p1,
        ns3:tp15 ;
    ns3:hasWorkingMode ns3:PulsedOperation .

ns3:QCL3 a ns3:QuantumCascadeLaser ;
    prov:wasAttributedTo <https://www.doi.org/10.1063/1.1554479> ;
    ns3:hasHeterostructure ns3:HS3 ;
    ns3:hasProperty ns3:f3,
        ns3:p2,
        ns3:tp16 ;
    ns3:hasWorkingMode ns3:PulsedOperation .

ns3:QCL4 a ns3:QuantumCascadeLaser ;
    prov:wasAttributedTo <https://www.doi.org/10.1063/1.3114418> ;
    ns3:hasHeterostructure ns3:HS4 ;
    ns3:hasProperty ns3:f4,
        ns3:p3,
        ns3:tp2 ;
    ns3:hasWorkingMode ns3:ContinousWaveOperation .

ns3:QCL5 a ns3:QuantumCascadeLaser ;
    prov:wasAttributedTo <https://www.doi.org/10.1063/1.4862177> ;
    ns3:hasHeterostructure ns3:HS5 ;
    ns3:hasProperty ns3:f5,
        ns3:tp3 ;
    ns3:hasWorkingMode ns3:ContinousWaveOperation .

ns3:QCL6 a ns3:QuantumCascadeLaser ;
    prov:wasAttributedTo <https://www.doi.org/10.1088/1367-2630/11/12/125022> ;
    ns3:hasHeterostructure ns3:HS6 ;
    ns3:hasProperty ns3:f6,
        ns3:tp4 ;
    ns3:hasWorkingMode ns3:ContinousWaveOperation .

ns3:QCL7 a ns3:QuantumCascadeLaser ;
    prov:wasAttributedTo <https://www.doi.org/10.1088/0256-307X/30/6/064201> ;
    ns3:hasHeterostructure ns3:HS7 ;
    ns3:hasProperty ns3:f7,
        ns3:p4,
        ns3:tp17,
        ns3:tp5 ;
    ns3:hasWorkingMode ns3:ContinousWaveOperation,
        ns3:PulsedOperation .

ns3:QCL8 a ns3:QuantumCascadeLaser ;
    prov:wasAttributedTo <https://www.doi.org/10.1088/1367-2630/18/12/123004> ;
    ns3:hasHeterostructure ns3:HS8 ;
    ns3:hasProperty ns3:f8,
        ns3:p5,
        ns3:tp6 ;
    ns3:hasWorkingMode ns3:ContinousWaveOperation .

ns3:QCL9 a ns3:QuantumCascadeLaser ;
    prov:wasAttributedTo <https://www.doi.org/10.1063/1.4766915> ;
    ns3:hasHeterostructure ns3:HS9 ;
    ns3:hasProperty ns3:f9,
        ns3:p6,
        ns3:tp7 ;
    ns3:hasWorkingMode ns3:ContinousWaveOperation .

ns3:URL a owl:DatatypeProperty ;
    rdfs:comment "URL represents that an academic article has the URL  in a string."@en ;
    rdfs:domain <http://purl.org/ontology/bibo/AcademicArticle> ;
    rdfs:range xsd:string .

ns3:basedOnMaterials a owl:ObjectProperty ;
    rdfs:label "based on materials"@en ;
    rdfs:comment "basedOnMaterials represents that the layer sequence is based on materials in the material composition of a heterostructure."@en ;
    rdfs:domain ns3:LayerSequence ;
    rdfs:range ns3:HeterostructureMaterials .

ns3:composedOf a owl:ObjectProperty ;
    rdfs:label "composed of"@en ;
    rdfs:comment "composedOf represents that materials are composed of atoms."@en ;
    rdfs:domain ns3:HeterostructureMaterials ;
    rdfs:range <https://ftp.ebi.ac.uk/pub/databases/chebi/ontology/#Atom> .

ns3:hasHeterostructure a owl:ObjectProperty ;
    rdfs:label "has heterostructure"@en ;
    rdfs:comment "has heterostructure represents the relationship between a quantum cascade laser and the heterostructural design it has."@en ;
    rdfs:domain ns3:QuantumCascadeLaser ;
    rdfs:range ns3:LaserHeterostructure .

ns3:hasLayerSequence a owl:ObjectProperty ;
    rdfs:label "has layer sequence"@en ;
    rdfs:comment "hasLayerSequence indicates the relationship between a heterostructure and the layer sequence it has."@en ;
    rdfs:domain ns3:LaserHeterostructure ;
    rdfs:range ns3:LayerSequence .

ns3:hasMaterials a owl:ObjectProperty ;
    rdfs:label "has materials"@en ;
    rdfs:comment "hasMaterials represents that a heterostructure has materials that form the heterostructure layer."@en ;
    rdfs:domain ns3:LaserHeterostructure .

ns3:hasProperty a owl:ObjectProperty ;
    rdfs:label "has property"@en ;
    rdfs:comment "hasProperty represents the relationship between a quantum cascade laser device and the property it has."@en ;
    rdfs:domain ns3:QuantumCascadeLaser ;
    rdfs:range mdo-core:Property .

ns3:hasWorkingMode a owl:ObjectProperty ;
    rdfs:label "has working mode"@en ;
    rdfs:comment "hasWorkingMode represents the relationship between a laser device and the working mode in which it is working."@en ;
    rdfs:domain ns3:QuantumCascadeLaser ;
    rdfs:range ns3:LaserWorkingMode .

ns3:matFormula a owl:DatatypeProperty ;
    rdfs:label "material formula"@en ;
    rdfs:comment "matFormula represents that materials have the fomula in a string. The formula indicates the material elemenst used and the number of atoms."@en ;
    rdfs:domain ns3:HeterostructureMaterials ;
    rdfs:range xsd:string .

ns3:relatesToMaterial a owl:ObjectProperty ;
    rdfs:label "relates to material"@en ;
    rdfs:comment "relatesToMaterial refers to the relationship between the heterostructure and the material space it comes from."@en ;
    rdfs:domain ns3:LaserHeterostructure ;
    rdfs:range emmo:Material .

ns3:sequence a owl:DatatypeProperty ;
    rdfs:comment "sequence represents that a layer sequence has a sequence in a string."@en ;
    rdfs:domain ns3:LayerSequence ;
    rdfs:range xsd:string .

ns2:hasQuantityValue a owl:ObjectProperty ;
    rdfs:label "has quantity value"@en ;
    rdfs:domain ns1:Quantity ;
    rdfs:range ns1:QuantityValue .

ns1:hasQuantityKind a owl:ObjectProperty ;
    rdfs:label "has quantity kind"@en ;
    rdfs:domain ns1:Quantity ;
    rdfs:range ns1:QuantityKind .

ns1:numericValue a owl:DatatypeProperty ;
    rdfs:domain ns1:QuantityValue ;
    rdfs:range xsd:float .

emmo:Material a owl:Class ;
    rdfs:label "EMMO:Material"@en .

<https://ftp.ebi.ac.uk/pub/databases/chebi/ontology/#Atom> a owl:Class ;
    rdfs:label "ChEBI:Atom"@en ;
    rdfs:comment "A chemical entity constituting the smallest component of an element having the chemical properties of the element."@en .

ns3:LS1 a ns3:LayerSequence ;
    ns3:basedOnMaterials ns3:M1 ;
    ns3:sequence "49/78/23/76/32/76/52/168" ;
    ns1:hasUnit <https://qudt.org/vocab/unit/ANGSTROM> .

ns3:LS10 a ns3:LayerSequence ;
    ns3:basedOnMaterials ns3:M10 ;
    ns3:sequence "217 /43 /111 /35 /132 /20/128 /51" ;
    ns1:hasUnit <https://qudt.org/vocab/unit/ANGSTROM> .

ns3:LS11 a ns3:LayerSequence ;
    ns3:basedOnMaterials ns3:M11 ;
    ns3:sequence "43/89/24.6/81.5/41/160" ;
    ns1:hasUnit <https://qudt.org/vocab/unit/ANGSTROM> .

ns3:LS12 a ns3:LayerSequence ;
    ns3:basedOnMaterials ns3:M12 ;
    ns3:sequence "9/79/25/66/41/156/33/90" ;
    ns1:hasUnit <https://qudt.org/vocab/unit/ANGSTROM> .

ns3:LS14 a ns3:LayerSequence ;
    ns3:basedOnMaterials ns3:M14 ;
    ns3:sequence "31/93/14/82/23/175/11/105/14/85/20/175/17/105" ;
    ns1:hasUnit <https://qudt.org/vocab/unit/ANGSTROM> .

ns3:LS2 a ns3:LayerSequence ;
    ns3:basedOnMaterials ns3:M2 ;
    ns3:sequence "4.24/8.48/3.11/11.02/2.54/7.91/4.24/16.67" ;
    ns1:hasUnit <https://qudt.org/vocab/unit/NanoM> .

ns3:LS3 a ns3:LayerSequence ;
    ns3:basedOnMaterials ns3:M3 ;
    ns3:sequence "54/78/24/64/38/148/24/94" ;
    ns1:hasUnit <https://qudt.org/vocab/unit/ANGSTROM> .

ns3:LS4 a ns3:LayerSequence ;
    ns3:basedOnMaterials ns3:M4 ;
    ns3:sequence "4.8/8.5/2.8/8.5/4.2/16.4" ;
    ns1:hasUnit <https://qudt.org/vocab/unit/NanoM> .

ns3:LS5 a ns3:LayerSequence ;
    ns3:basedOnMaterials ns3:M5 ;
    ns3:sequence "35/48/8/38.9/9/72/2/85.6/5/66" ;
    ns1:hasUnit <https://qudt.org/vocab/unit/ANGSTROM> .

ns3:LS6 a ns3:LayerSequence ;
    ns3:basedOnMaterials ns3:M6 ;
    ns3:sequence "5.5/11.0/1.8/11.5/3.8/9.4/4.2/18.4" ;
    ns1:hasUnit <https://qudt.org/vocab/unit/NanoM> .

ns3:LS7 a ns3:LayerSequence ;
    ns3:basedOnMaterials ns3:M7 ;
    ns3:sequence "4.0/12/0.5/22.3/0.8/21.5/0.9/17.8/1/14.5/1.3/13.2?/2.2/13.4/2.8/17" ;
    ns1:hasUnit <https://qudt.org/vocab/unit/NanoM> .

ns3:LS8 a ns3:LayerSequence ;
    ns3:basedOnMaterials ns3:M8 ;
    ns3:sequence "5.1/9.3/1.0/10.5/3.3/8.7/4.2/16.5" ;
    ns1:hasUnit <https://qudt.org/vocab/unit/NanoM> .

ns3:LS9 a ns3:LayerSequence ;
    ns3:basedOnMaterials ns3:M9 ;
    ns3:sequence "2.0/20.3/2.0/3.0/14.4/1.0/13.5/3.0" ;
    ns1:hasUnit <https://qudt.org/vocab/unit/NanoM> .

ns3:f1 ns3:relatesToHeterostructure ns3:HS1 ;
    ns2:hasQuantityValue ns3:fv1 ;
    ns1:hasQuantityKind <https://qudt.org/vocab/quantitykind/Frequency> .

ns3:f2 ns3:relatesToHeterostructure ns3:HS2 ;
    ns2:hasQuantityValue ns3:fv2 ;
    ns1:hasQuantityKind <https://qudt.org/vocab/quantitykind/Frequency> .

ns3:f3 ns3:relatesToHeterostructure ns3:HS3 ;
    ns2:hasQuantityValue ns3:fv3 ;
    ns1:hasQuantityKind <https://qudt.org/vocab/quantitykind/Frequency> .

ns3:f4 ns3:relatesToHeterostructure ns3:HS4 ;
    ns2:hasQuantityValue ns3:fv4 ;
    ns1:hasQuantityKind <https://qudt.org/vocab/quantitykind/Frequency> .

ns3:f5 ns3:relatesToHeterostructure ns3:HS5 ;
    ns2:hasQuantityValue ns3:fv5 ;
    ns1:hasQuantityKind <https://qudt.org/vocab/quantitykind/Frequency> .

ns3:f6 ns3:relatesToHeterostructure ns3:HS6 ;
    ns2:hasQuantityValue ns3:fv6 ;
    ns1:hasQuantityKind <https://qudt.org/vocab/quantitykind/Frequency> .

ns3:f7 ns3:relatesToHeterostructure ns3:HS7 ;
    ns2:hasQuantityValue ns3:fv7 ;
    ns1:hasQuantityKind <https://qudt.org/vocab/quantitykind/Frequency> .

ns3:f8 ns3:relatesToHeterostructure ns3:HS8 ;
    ns2:hasQuantityValue ns3:fv8 ;
    ns1:hasQuantityKind <https://qudt.org/vocab/quantitykind/Frequency> .

ns3:f9 ns3:relatesToHeterostructure ns3:HS9 ;
    ns2:hasQuantityValue ns3:fv9 ;
    ns1:hasQuantityKind <https://qudt.org/vocab/quantitykind/Frequency> .

ns3:fv1 ns1:hasUnit <https://qudt.org/vocab/unit/TeraHZ> ;
    ns1:numericValue "1.9" .

ns3:fv2 ns1:hasUnit <https://qudt.org/vocab/unit/TeraHZ> ;
    ns1:numericValue "2.1" .

ns3:fv3 ns1:hasUnit <https://qudt.org/vocab/unit/TeraHZ> ;
    ns1:numericValue "3.44" .

ns3:fv4 ns1:hasUnit <https://qudt.org/vocab/unit/TeraHZ> ;
    ns1:numericValue "3.9" .

ns3:fv5 ns1:hasUnit <https://qudt.org/vocab/unit/TeraHZ> ;
    ns1:numericValue "2.67" .

ns3:fv6 ns1:hasUnit <https://qudt.org/vocab/unit/TeraHZ> ;
    ns1:numericValue "3" .

ns3:fv7 ns1:hasUnit <https://qudt.org/vocab/unit/TeraHZ> ;
    ns1:numericValue "3.2" .

ns3:fv8 ns1:hasUnit <https://qudt.org/vocab/unit/TeraHZ> ;
    ns1:numericValue "4.7" .

ns3:fv9 ns1:hasUnit <https://qudt.org/vocab/unit/TeraHZ> ;
    ns1:numericValue "3.3" .

ns3:p1 ns3:relatesToHeterostructure ns3:HS2 ;
    ns2:hasQuantityValue ns3:pv1 ;
    ns1:hasQuantityKind <https://qudt.org/vocab/quantitykind/Power> .

ns3:p2 ns3:relatesToHeterostructure ns3:HS3 ;
    ns2:hasQuantityValue ns3:pv2 ;
    ns1:hasQuantityKind <https://qudt.org/vocab/quantitykind/Power> .

ns3:p3 ns3:relatesToHeterostructure ns3:HS4 ;
    ns2:hasQuantityValue ns3:pv3 ;
    ns1:hasQuantityKind <https://qudt.org/vocab/quantitykind/Power> .

ns3:p4 ns3:relatesToHeterostructure ns3:HS7 ;
    ns2:hasQuantityValue ns3:pv4 ;
    ns1:hasQuantityKind <https://qudt.org/vocab/quantitykind/Power> .

ns3:p5 ns3:relatesToHeterostructure ns3:HS8 ;
    ns2:hasQuantityValue ns3:pv5 ;
    ns1:hasQuantityKind <https://qudt.org/vocab/quantitykind/Power> .

ns3:p6 ns3:relatesToHeterostructure ns3:HS9 ;
    ns2:hasQuantityValue ns3:pv6 ;
    ns1:hasQuantityKind <https://qudt.org/vocab/quantitykind/Power> .

ns3:p7 ns3:relatesToHeterostructure ns3:HS11 ;
    ns2:hasQuantityValue ns3:pv7 ;
    ns1:hasQuantityKind <https://qudt.org/vocab/quantitykind/Power> .

ns3:p8 ns3:relatesToHeterostructure ns3:HS13 ;
    ns2:hasQuantityValue ns3:pv8 ;
    ns1:hasQuantityKind <https://qudt.org/vocab/quantitykind/Power> .

ns3:p9 ns3:relatesToHeterostructure ns3:HS15 ;
    ns2:hasQuantityValue ns3:pv9 ;
    ns1:hasQuantityKind <https://qudt.org/vocab/quantitykind/Power> .

ns3:pv1 ns1:hasUnit <https://qudt.org/vocab/unit/MilliW> ;
    ns1:numericValue "10" .

ns3:pv2 ns1:hasUnit <https://qudt.org/vocab/unit/MilliW> ;
    ns1:numericValue "2.5" .

ns3:pv3 ns1:hasUnit <https://qudt.org/vocab/unit/MilliW> ;
    ns1:numericValue "62" .

ns3:pv4 ns1:hasUnit <https://qudt.org/vocab/unit/MilliW> ;
    ns1:numericValue "62" .

ns3:pv5 ns1:hasUnit <https://qudt.org/vocab/unit/MilliW> ;
    ns1:numericValue "200" .

ns3:pv6 ns1:hasUnit <https://qudt.org/vocab/unit/MilliW> ;
    ns1:numericValue "9" .

ns3:pv7 ns1:hasUnit <https://qudt.org/vocab/unit/MilliW> ;
    ns1:numericValue "38" .

ns3:pv8 ns1:hasUnit <https://qudt.org/vocab/unit/MilliW> ;
    ns1:numericValue "100" .

ns3:pv9 ns1:hasUnit <https://qudt.org/vocab/unit/MilliW> ;
    ns1:numericValue "200" .

ns3:tp1 ns3:correspondsToWorkingMode ns3:ContinousWaveOperation ;
    ns3:relatesToHeterostructure ns3:HS1 ;
    ns2:hasQuantityValue ns3:tv1 ;
    ns1:hasQuantityKind <https://qudt.org/vocab/quantitykind/Temperature> .

ns3:tp10 ns3:correspondsToWorkingMode ns3:ContinousWaveOperation ;
    ns3:relatesToHeterostructure ns3:HS12 ;
    ns2:hasQuantityValue ns3:tv10 ;
    ns1:hasQuantityKind <https://qudt.org/vocab/quantitykind/Temperature> .

ns3:tp11 ns3:correspondsToWorkingMode ns3:ContinousWaveOperation ;
    ns3:relatesToHeterostructure ns3:HS13 ;
    ns2:hasQuantityValue ns3:tv11 ;
    ns1:hasQuantityKind <https://qudt.org/vocab/quantitykind/Temperature> .

ns3:tp12 ns3:correspondsToWorkingMode ns3:ContinousWaveOperation ;
    ns3:relatesToHeterostructure ns3:HS14 ;
    ns2:hasQuantityValue ns3:tv12 ;
    ns1:hasQuantityKind <https://qudt.org/vocab/quantitykind/Temperature> .

ns3:tp13 ns3:correspondsToWorkingMode ns3:ContinousWaveOperation ;
    ns3:relatesToHeterostructure ns3:HS15 ;
    ns2:hasQuantityValue ns3:tv13 ;
    ns1:hasQuantityKind <https://qudt.org/vocab/quantitykind/Temperature> .

ns3:tp14 ns3:correspondsToWorkingMode ns3:PulsedOperation ;
    ns3:relatesToHeterostructure ns3:HS1 ;
    ns2:hasQuantityValue ns3:tv14 ;
    ns1:hasQuantityKind <https://qudt.org/vocab/quantitykind/Temperature> .

ns3:tp15 ns3:correspondsToWorkingMode ns3:PulsedOperation ;
    ns3:relatesToHeterostructure ns3:HS2 ;
    ns2:hasQuantityValue ns3:tv15 ;
    ns1:hasQuantityKind <https://qudt.org/vocab/quantitykind/Temperature> .

ns3:tp16 ns3:correspondsToWorkingMode ns3:PulsedOperation ;
    ns3:relatesToHeterostructure ns3:HS3 ;
    ns2:hasQuantityValue ns3:tv16 ;
    ns1:hasQuantityKind <https://qudt.org/vocab/quantitykind/Temperature> .

ns3:tp17 ns3:correspondsToWorkingMode ns3:PulsedOperation ;
    ns3:relatesToHeterostructure ns3:HS7 ;
    ns2:hasQuantityValue ns3:tv17 ;
    ns1:hasQuantityKind <https://qudt.org/vocab/quantitykind/Temperature> .

ns3:tp18 ns3:correspondsToWorkingMode ns3:PulsedOperation ;
    ns3:relatesToHeterostructure ns3:HS14 ;
    ns2:hasQuantityValue ns3:tv18 ;
    ns1:hasQuantityKind <https://qudt.org/vocab/quantitykind/Temperature> .

ns3:tp2 ns3:correspondsToWorkingMode ns3:ContinousWaveOperation ;
    ns3:relatesToHeterostructure ns3:HS4 ;
    ns2:hasQuantityValue ns3:tv2 ;
    ns1:hasQuantityKind <https://qudt.org/vocab/quantitykind/Temperature> .

ns3:tp3 ns3:correspondsToWorkingMode ns3:ContinousWaveOperation ;
    ns3:relatesToHeterostructure ns3:HS5 ;
    ns2:hasQuantityValue ns3:tv3 ;
    ns1:hasQuantityKind <https://qudt.org/vocab/quantitykind/Temperature> .

ns3:tp4 ns3:correspondsToWorkingMode ns3:ContinousWaveOperation ;
    ns3:relatesToHeterostructure ns3:HS6 ;
    ns2:hasQuantityValue ns3:tv4 ;
    ns1:hasQuantityKind <https://qudt.org/vocab/quantitykind/Temperature> .

ns3:tp5 ns3:correspondsToWorkingMode ns3:ContinousWaveOperation ;
    ns3:relatesToHeterostructure ns3:HS7 ;
    ns2:hasQuantityValue ns3:tv5 ;
    ns1:hasQuantityKind <https://qudt.org/vocab/quantitykind/Temperature> .

ns3:tp6 ns3:correspondsToWorkingMode ns3:ContinousWaveOperation ;
    ns3:relatesToHeterostructure ns3:HS8 ;
    ns2:hasQuantityValue ns3:tv6 ;
    ns1:hasQuantityKind <https://qudt.org/vocab/quantitykind/Temperature> .

ns3:tp7 ns3:correspondsToWorkingMode ns3:ContinousWaveOperation ;
    ns3:relatesToHeterostructure ns3:HS9 ;
    ns2:hasQuantityValue ns3:tv7 ;
    ns1:hasQuantityKind <https://qudt.org/vocab/quantitykind/Temperature> .

ns3:tp8 ns3:correspondsToWorkingMode ns3:ContinousWaveOperation ;
    ns3:relatesToHeterostructure ns3:HS10 ;
    ns2:hasQuantityValue ns3:tv8 ;
    ns1:hasQuantityKind <https://qudt.org/vocab/quantitykind/Temperature> .

ns3:tp9 ns3:correspondsToWorkingMode ns3:ContinousWaveOperation ;
    ns3:relatesToHeterostructure ns3:HS11 ;
    ns2:hasQuantityValue ns3:tv9 ;
    ns1:hasQuantityKind <https://qudt.org/vocab/quantitykind/Temperature> .

ns3:tv1 ns1:hasUnit <https://qudt.org/vocab/unit/K> ;
    ns1:numericValue "95" .

ns3:tv10 ns1:hasUnit <https://qudt.org/vocab/unit/K> ;
    ns1:numericValue "178" .

ns3:tv11 ns1:hasUnit <https://qudt.org/vocab/unit/K> ;
    ns1:numericValue "45" .

ns3:tv12 ns1:hasUnit <https://qudt.org/vocab/unit/K> ;
    ns1:numericValue "105" .

ns3:tv13 ns1:hasUnit <https://qudt.org/vocab/unit/K> ;
    ns1:numericValue "210.5" .

ns3:tv14 ns1:hasUnit <https://qudt.org/vocab/unit/K> ;
    ns1:numericValue "110" .

ns3:tv15 ns1:hasUnit <https://qudt.org/vocab/unit/K> ;
    ns1:numericValue "144" .

ns3:tv16 ns1:hasUnit <https://qudt.org/vocab/unit/K> ;
    ns1:numericValue "65" .

ns3:tv17 ns1:hasUnit <https://qudt.org/vocab/unit/K> ;
    ns1:numericValue "85" .

ns3:tv18 ns1:hasUnit <https://qudt.org/vocab/unit/K> ;
    ns1:numericValue "138" .

ns3:tv2 ns1:hasUnit <https://qudt.org/vocab/unit/K> ;
    ns1:numericValue "186" .

ns3:tv3 ns1:hasUnit <https://qudt.org/vocab/unit/K> ;
    ns1:numericValue "151" .

ns3:tv4 ns1:hasUnit <https://qudt.org/vocab/unit/K> ;
    ns1:numericValue "100" .

ns3:tv5 ns1:hasUnit <https://qudt.org/vocab/unit/K> ;
    ns1:numericValue "60" .

ns3:tv6 ns1:hasUnit <https://qudt.org/vocab/unit/K> ;
    ns1:numericValue "150" .

ns3:tv7 ns1:hasUnit <https://qudt.org/vocab/unit/K> ;
    ns1:numericValue "142" .

ns3:tv8 ns1:hasUnit <https://qudt.org/vocab/unit/K> ;
    ns1:numericValue "195" .

ns3:tv9 ns1:hasUnit <https://qudt.org/vocab/unit/K> ;
    ns1:numericValue "200" .

<https://opg.optica.org/oe/fulltext.cfm?uri=oe-23-15-19689&id=323020> a <http://purl.org/ontology/bibo/AcademicArticle> ;
    ns3:DOI "10.1364/OE.23.019689 " ;
    ns3:URL "https://opg.optica.org/oe/fulltext.cfm?uri=oe-23-15-19689&id=323020" .

<https://www.doi.org/10.1063/1.1554479> a <http://purl.org/ontology/bibo/AcademicArticle> ;
    ns3:DOI "10.1063/1.1554479" ;
    ns3:URL "https://www.doi.org/10.1063/1.1554479" .

<https://www.doi.org/10.1063/1.2189671> a <http://purl.org/ontology/bibo/AcademicArticle> ;
    ns3:DOI "10.1063/1.2189671" ;
    ns3:URL "https://www.doi.org/10.1063/1.2189671" .

<https://www.doi.org/10.1063/1.2216112> a <http://purl.org/ontology/bibo/AcademicArticle> ;
    ns3:DOI "10.1063/1.2216112" ;
    ns3:URL "https://www.doi.org/10.1063/1.2216112" .

<https://www.doi.org/10.1063/1.2737129> a <http://purl.org/ontology/bibo/AcademicArticle> ;
    ns3:DOI "10.1063/1.2737129" ;
    ns3:URL "https://www.doi.org/10.1063/1.2737129" .

<https://www.doi.org/10.1063/1.3114418> a <http://purl.org/ontology/bibo/AcademicArticle> ;
    ns3:DOI "10.1063/1.3114418" ;
    ns3:URL "https://www.doi.org/10.1063/1.3114418" .

<https://www.doi.org/10.1063/1.4766915> a <http://purl.org/ontology/bibo/AcademicArticle> ;
    ns3:DOI "10.1063/1.4766915" ;
    ns3:URL "https://www.doi.org/10.1063/1.4766915" .

<https://www.doi.org/10.1063/1.4862177> a <http://purl.org/ontology/bibo/AcademicArticle> ;
    ns3:DOI "10.1063/1.4862177" ;
    ns3:URL "https://www.doi.org/10.1063/1.4862177" .

<https://www.doi.org/10.1063/1.5110305> a <http://purl.org/ontology/bibo/AcademicArticle> ;
    ns3:DOI "10.1063/1.5110305" ;
    ns3:URL "https://www.doi.org/10.1063/1.5110305" .

<https://www.doi.org/10.1088/0256-307X/30/6/064201> a <http://purl.org/ontology/bibo/AcademicArticle> ;
    ns3:DOI "10.1088/0256-307X/30/6/064201" ;
    ns3:URL "https://www.doi.org/10.1088/0256-307X/30/6/064201" .

<https://www.doi.org/10.1088/1367-2630/11/12/125022> a <http://purl.org/ontology/bibo/AcademicArticle> ;
    ns3:DOI "10.1088/1367-2630/11/12/125022" ;
    ns3:URL "https://www.doi.org/10.1088/1367-2630/11/12/125022" .

<https://www.doi.org/10.1088/1367-2630/17/2/023050> a <http://purl.org/ontology/bibo/AcademicArticle> ;
    ns3:DOI "10.1088/1367-2630/17/2/023050" ;
    ns3:URL "https://www.doi.org/10.1088/1367-2630/17/2/023050" .

<https://www.doi.org/10.1088/1367-2630/18/12/123004> a <http://purl.org/ontology/bibo/AcademicArticle> ;
    ns3:DOI "10.1088/1367-2630/18/12/123004" ;
    ns3:URL "https://www.doi.org/10.1088/1367-2630/18/12/123004" .

<https://www.doi.org/10.1364/OE.16.003242> a <http://purl.org/ontology/bibo/AcademicArticle> ;
    ns3:DOI "10.1364/OE.16.003242" ;
    ns3:URL "https://www.doi.org/10.1364/OE.16.003242" .

<https://www.doi.org/10.1364/OE.20.003866> a <http://purl.org/ontology/bibo/AcademicArticle> ;
    ns3:DOI "10.1364/OE.20.003866" ;
    ns3:URL "https://www.doi.org/10.1364/OE.20.003866" .

<https://www.w3.org/TR/prov-o/#Agent> a owl:Class ;
    rdfs:comment "An agent is something that bears some form of responsibility for an activity taking place, for the existence of an entity, or for another agent's activity."@en .

ns3:HS10 a ns3:LaserHeterostructure ;
    ns3:hasDesignType ns3:BoundToContinum ;
    ns3:hasLayerSequence ns3:LS10 ;
    ns3:hasMaterials ns3:M10 .

ns3:M1 a ns3:HeterostructureMaterials ;
    ns3:matFormula "GaAs/Al0.15Ga0.85As" .

ns3:M10 a ns3:HeterostructureMaterials ;
    ns3:matFormula "In 0.53 Ga 0.47 As/Al 0.17In 0.52 Ga 0.31 As" .

ns3:M11 a ns3:HeterostructureMaterials ;
    ns3:matFormula "GaAs/Al0.15Ga0.85As" .

ns3:M12 a ns3:HeterostructureMaterials ;
    ns3:matFormula "GaAs/Al0.15Ga0.85As" .

ns3:M14 a ns3:HeterostructureMaterials ;
    ns3:matFormula "GaAs/Al0.3Ga0.7As" .

ns3:M2 a ns3:HeterostructureMaterials ;
    ns3:matFormula "GaAs/Al0.15Ga0.85As" .

ns3:M3 a ns3:HeterostructureMaterials ;
    ns3:matFormula "GaAs/Al0.15Ga0.85As" .

ns3:M4 a ns3:HeterostructureMaterials ;
    ns3:matFormula "GaAs/Al0.15Ga0.85As" .

ns3:M5 a ns3:HeterostructureMaterials ;
    ns3:matFormula "GaAs/Al0.25Ga0.75As" .

ns3:M6 a ns3:HeterostructureMaterials ;
    ns3:matFormula "GaAs/Al0.15Ga0.85As" .

ns3:M7 a ns3:HeterostructureMaterials ;
    ns3:matFormula "GaAs/Al0.15Ga0.85As" .

ns3:M8 a ns3:HeterostructureMaterials ;
    ns3:matFormula "GaAs/Al0.15Ga0.85As" .

ns3:M9 a ns3:HeterostructureMaterials ;
    ns3:matFormula "In0.53Ga0.47As/GaAs0.51Sb0.49" .

ns3:correspondsToWorkingMode a owl:ObjectProperty ;
    rdfs:label "corresponds to working mode"@en ;
    rdfs:comment "correspondsToWorkingMode represents the relationship between a property and the laser working mode under which it was obtained."@en ;
    rdfs:domain mdo-core:Property ;
    rdfs:range ns3:LaserWorkingMode .

ns3:f10 ns3:relatesToHeterostructure ns3:HS11 ;
    ns2:hasQuantityValue ns3:f10 ;
    ns1:hasQuantityKind <https://qudt.org/vocab/quantitykind/Frequency> ;
    ns1:hasUnit <https://qudt.org/vocab/unit/TeraHZ> ;
    ns1:numericValue "3.2" .

ns3:f11 ns3:relatesToHeterostructure ns3:HS12 ;
    ns2:hasQuantityValue ns3:f11 ;
    ns1:hasQuantityKind <https://qudt.org/vocab/quantitykind/Frequency> ;
    ns1:hasUnit <https://qudt.org/vocab/unit/TeraHZ> ;
    ns1:numericValue "3" .

ns3:f12 ns3:relatesToHeterostructure ns3:HS13 ;
    ns2:hasQuantityValue ns3:f12 ;
    ns1:hasQuantityKind <https://qudt.org/vocab/quantitykind/Frequency> ;
    ns1:hasUnit <https://qudt.org/vocab/unit/TeraHZ> ;
    ns1:numericValue "2.83" .

ns3:f13 ns3:relatesToHeterostructure ns3:HS15 ;
    ns2:hasQuantityValue ns3:f13 ;
    ns1:hasQuantityKind <https://qudt.org/vocab/quantitykind/Frequency> ;
    ns1:hasUnit <https://qudt.org/vocab/unit/TeraHZ> ;
    ns1:numericValue "3.95" .

ns3:hasDesignType a owl:ObjectProperty ;
    rdfs:label "has design type"@en ;
    rdfs:comment "hasDesignType indicates the relatioship between the laser heterostructure and the desgn type on whch it is based."@en ;
    rdfs:domain ns3:LaserHeterostructure ;
    rdfs:range ns3:LaserDesignType .

ns3:BoundToContinum a owl:NamedIndividual,
        ns3:LaserDesignType ;
    rdfs:label "bound to continum"@en ;
    rdfs:comment "A laser design where the sequence of material in the active region is made with more or less increasing width of layers in the multistack of material."@en .

ns3:DoubleResonantPhonon a owl:NamedIndividual,
        ns3:LaserDesignType ;
    rdfs:label "double resonant phonon"@en ;
    rdfs:comment "A laser design where two quantum well are resonant."@en .

ns3:HS12 a ns3:LaserHeterostructure ;
    ns3:hasDesignType ns3:DoubleResonantPhonon ;
    ns3:hasLayerSequence ns3:LS12 ;
    ns3:hasMaterials ns3:M12 .

ns3:HS14 a ns3:LaserHeterostructure ;
    ns3:hasDesignType ns3:LOPhononDepopulation ;
    ns3:hasLayerSequence ns3:LS14 ;
    ns3:hasMaterials ns3:M14 .

ns3:HS5 a ns3:LaserHeterostructure ;
    ns3:hasDesignType ns3:LOPhononDepopulation ;
    ns3:hasLayerSequence ns3:LS5 ;
    ns3:hasMaterials ns3:M5 .

ns3:HS6 a ns3:LaserHeterostructure ;
    ns3:hasDesignType ns3:BoundToContinum ;
    ns3:hasLayerSequence ns3:LS6 ;
    ns3:hasMaterials ns3:M6 .

ns1:Quantity a owl:Class ;
    rdfs:comment "A quantity is the measurement of an observable property of a particular object, event, or physical system."@en .

ns3:HS1 a ns3:LaserHeterostructure ;
    ns3:hasDesignType ns3:LOPhononDepopulation ;
    ns3:hasLayerSequence ns3:LS1 ;
    ns3:hasMaterials ns3:M1 .

ns3:HS11 a ns3:LaserHeterostructure ;
    ns3:hasDesignType ns3:LOPhononDepopulation ;
    ns3:hasLayerSequence ns3:LS11 ;
    ns3:hasMaterials ns3:M11 .

ns3:HS13 a ns3:LaserHeterostructure .

ns3:HS15 a ns3:LaserHeterostructure .

ns3:HS2 a ns3:LaserHeterostructure ;
    ns3:hasDesignType ns3:DoubleResonantPhonon ;
    ns3:hasLayerSequence ns3:LS2 ;
    ns3:hasMaterials ns3:M2 .

ns3:HS3 a ns3:LaserHeterostructure ;
    ns3:hasDesignType ns3:LOPhononDepopulation ;
    ns3:hasLayerSequence ns3:LS3 ;
    ns3:hasMaterials ns3:M3 .

ns3:HS4 a ns3:LaserHeterostructure ;
    ns3:hasDesignType ns3:DoubleResonantPhonon ;
    ns3:hasLayerSequence ns3:LS4 ;
    ns3:hasMaterials ns3:M4 .

ns3:HS8 a ns3:LaserHeterostructure ;
    ns3:hasDesignType ns3:LOPhononDepopulation ;
    ns3:hasLayerSequence ns3:LS8 ;
    ns3:hasMaterials ns3:M8 .

ns3:HS9 a ns3:LaserHeterostructure ;
    ns3:hasDesignType ns3:LOPhononDepopulation ;
    ns3:hasLayerSequence ns3:LS9 ;
    ns3:hasMaterials ns3:M9 .

ns1:QuantityKind a owl:Class ;
    rdfs:label "Quantity Kind"@en ;
    rdfs:comment "A Quantity Kind is any observable property that can be measured and quantified numerically. Familiar examples include physical properties such as length, mass, time, force, energy, power, electric charge, etc."@en .

ns3:HS7 a ns3:LaserHeterostructure ;
    ns3:hasDesignType ns3:BoundToContinum ;
    ns3:hasLayerSequence ns3:LS7 ;
    ns3:hasMaterials ns3:M7 .

mdo-core:Property a owl:Class ;
    rdfs:label "Property"@en ;
    rdfs:comment "A property in materials design is data pertaining to at least one material or materials system, representing a quantifiable aspect of one material or materials system."@en ;
    rdfs:subClassOf [ a owl:Class ;
            owl:intersectionOf ( [ a owl:Restriction ;
                        owl:allValuesFrom ns3:LaserWorkingMode ;
                        owl:onProperty ns3:correspondsToWorkingMode ] [ a owl:Restriction ;
                        owl:onClass ns3:LaserWorkingMode ;
                        owl:onProperty ns3:correspondsToWorkingMode ;
                        owl:qualifiedCardinality "1"^^xsd:nonNegativeInteger ] ) ],
        ns1:Quantity .

ns3:LaserDesignType a owl:Class ;
    rdfs:label "Laser Design Type"@en ;
    rdfs:comment "Represents the geometrical aspects of the laser design."@en .

ns3:LaserWorkingMode a owl:Class ;
    rdfs:label "Laser Working Mode"@en ;
    rdfs:comment "Refers to the nature in which the laser beams are emmitted."@en .

ns1:QuantityValue a owl:Class ;
    rdfs:label "Quantity Value"@en .

ns1:Unit a owl:Class ;
    rdfs:label "Unit"@en ;
    rdfs:comment "A unit of measure, or unit, is a particular quantity value that has been chosen as a scale for measuring other quantities the same kind (more generally of equivalent dimension)."@en .

<https://qudt.org/vocab/unit/NanoM> a ns1:Unit .

ns3:LOPhononDepopulation a owl:NamedIndividual,
        ns3:LaserDesignType ;
    rdfs:label "LO Phonon Depopulation"@en ;
    rdfs:comment "LO Phonon depopulation refers to the laser design where the sequence of material in the active region is designed to provide laser effect from longitudinal Optical Phonons."@en .

<https://qudt.org/vocab/unit/ANGSTROM> a ns1:Unit .

ns3:OpticalPower a owl:NamedIndividual,
        mdo-core:Property ;
    rdfs:label "optical power"@en ;
    rdfs:comment "OpticalPower refers to the laser output power."@en .

ns3:PowerValue a owl:NamedIndividual,
        ns1:QuantityValue ;
    rdfs:label "power value"@en ;
    rdfs:comment "PowerValue refers to the quanity value of the laser optical power."@en .

<https://qudt.org/vocab/quantitykind/Power> a ns1:QuantityKind .

ns3:PulsedOperation a owl:NamedIndividual,
        ns3:LaserWorkingMode ;
    rdfs:label "pulsed operation"@en ;
    rdfs:comment "Pulse operation  refers to the laser operation mode in which laser beams are emitted in pulses."@en .

ns3:FrequencyValue a owl:NamedIndividual,
        ns1:QuantityValue ;
    rdfs:label "lasing frequency value"@en ;
    rdfs:comment "Frequency Value refers to the quantity value of the laser lasing frequency."@en .

ns3:LasingFrequency a owl:NamedIndividual,
        mdo-core:Property ;
    rdfs:label "lasing frequency"@en ;
    rdfs:comment "LasingFrequency refers to the frequency at which the quantum cascade lasers emits the laser beams."@en .

<https://qudt.org/vocab/quantitykind/Frequency> a ns1:QuantityKind .

ns3:HeterostructureMaterials a owl:Class ;
    rdfs:label "Heterostructure Materials"@en ;
    rdfs:comment "Heterostructure Materials refers to the materials forming the heterostructure layer."@en .

ns3:WorkingTempValue a owl:NamedIndividual,
        ns1:QuantityValue ;
    rdfs:label "working temperature value"@en ;
    rdfs:comment "WorkingTempValue refers to the quantity value of the laser working/operation temperature."@en .

ns3:WorkingTemperature a owl:NamedIndividual,
        mdo-core:Property ;
    rdfs:label "working temperature"@en ;
    rdfs:comment "WorkingTemperature refers to the operation temperature under which the quantum cascade laser emmits the laser beams."@en .

<https://qudt.org/vocab/quantitykind/Temperature> a ns1:QuantityKind .

<https://qudt.org/vocab/unit/K> a ns1:Unit .

ns3:LayerSequence a owl:Class ;
    rdfs:label "Layer Sequence"@en ;
    rdfs:comment "Reprsents the sequence and thickness of materials composing the heterostructure."@en .

ns3:QuantumCascadeLaser a owl:Class ;
    rdfs:label "Quantum Cascade Laser"@en ;
    rdfs:comment "Semiconductor lasers that operate in the mid to far-infrared region."@en .

ns3:LaserHeterostructure a owl:Class ;
    rdfs:label "Laser Heterostructure"@en ;
    rdfs:comment "A layered material composed of different semiconductor materials."@en ;
    rdfs:subClassOf [ a owl:Class ;
            owl:intersectionOf ( [ a owl:Restriction ;
                        owl:allValuesFrom ns3:LaserDesignType ;
                        owl:onProperty ns3:hasDesignType ] [ a owl:Restriction ;
                        owl:onClass ns3:LaserDesignType ;
                        owl:onProperty ns3:hasDesignType ;
                        owl:qualifiedCardinality "1"^^xsd:nonNegativeInteger ] ) ] .

<http://purl.org/ontology/bibo/AcademicArticle> a owl:Class ;
    rdfs:label "Academic Article"@en ;
    rdfs:comment "A scholarly academic article, typically published in a journal."@en ;
    rdfs:subClassOf <https://www.w3.org/TR/prov-o/#Agent> .

ns3:ContinousWaveOperation a owl:NamedIndividual,
        ns3:LaserWorkingMode ;
    rdfs:label "continous wave operation"@en ;
    rdfs:comment "Continous Wave Operation refers to the laser operation mode in which laser beams are emitted continously."@en .

