@prefix dcterms: <http://purl.org/dc/terms/> .
@prefix emmo: <http://emmo.info/domains/emmo-material.owl#> .
@prefix mdo-core: <https://w3id.org/mdo/core/> .
@prefix ns1: <https://github.com/DeperiasKerre/qcl_Onto/blob/main/qclontology/version-1.0/qclonto.owl#> .
@prefix ns2: <https://qudt.org/schema/qudt/> .
@prefix ns3: <http://qudt.org/schema/qudt/> .
@prefix ns4: <https://qudt.org/schema/qudt#> .
@prefix owl: <http://www.w3.org/2002/07/owl#> .
@prefix prov: <http://www.w3.org/ns/prov#> .
@prefix rdf: <http://www.w3.org/1999/02/22-rdf-syntax-ns#> .
@prefix rdfs: <http://www.w3.org/2000/01/rdf-schema#> .
@prefix vann: <http://purl.org/vocab/vann/> .
@prefix xsd: <http://www.w3.org/2001/XMLSchema#> .

dcterms:contributor a owl:AnnotationProperty .

dcterms:created a owl:AnnotationProperty .

dcterms:creator a owl:AnnotationProperty .

dcterms:license a owl:AnnotationProperty .

dcterms:title a owl:AnnotationProperty .

vann:preferredNamespacePrefix a owl:AnnotationProperty .

vann:preferredNamespaceUri a owl:AnnotationProperty .

ns3:hasUnit a owl:ObjectProperty ;
    rdfs:label "has unit"@en ;
    rdfs:comment "hasUnit represents that a quantity value has a unit."@en ;
    rdfs:domain ns1:LayerSequence,
        ns2:QuantityValue .

prov:wasAttributedTo a owl:ObjectProperty ;
    rdfs:comment "wasAttributedTo represents the relationship  quantum cascade laser device and the scientific article documenting its design and performance properties."@en ;
    rdfs:domain ns1:QuantumCascadeLaser .

ns1: a owl:Ontology ;
    dcterms:contributor "Anne Laurent",
        "Dicskson Owuor",
        "Kenneth Maussang" ;
    dcterms:created "2023-10-16" ;
    dcterms:creator "Deperias Kerre" ;
    dcterms:license "https://github.com/DeperiasKerre/qcl_Onto/blob/main/LICENSE" ;
    dcterms:title "An Ontology of Properties in the Quantum Cascade Laser Domain"@en ;
    vann:preferredNamespacePrefix "QpOnto"@en ;
    vann:preferredNamespaceUri "https://github.com/DeperiasKerre/qcl_Onto/blob/main/qclontology/version-1.0/qclonto.owl#"@en ;
    rdfs:comment "This is an ontological representation of properties in the quantum cascade laser domain."@en ;
    rdfs:seeAlso "https://github.com/DeperiasKerre/qcl_Onto" ;
    owl:versionIRI <https://github.com/DeperiasKerre/qcl_Onto/tree/main/qclontology/version-1.0> ;
    owl:versionInfo "1.0" .

ns1:AuthorName a owl:DatatypeProperty ;
    rdfs:comment "AuthorName represents that an academic article has the author name in a string."@en ;
    rdfs:domain <http://purl.org/ontology/bibo/AcademicArticle> ;
    rdfs:range xsd:string .

ns1:DOI a owl:DatatypeProperty ;
    rdfs:comment "DOI represents that an academic article has the DOI in a string."@en ;
    rdfs:domain <http://purl.org/ontology/bibo/AcademicArticle> ;
    rdfs:range xsd:string .

ns1:HS10 a ns1:LaserHeterostructure ;
    ns1:hasDesignType ns1:BoundToContinum ;
    ns1:hasLayerSequence ns1:LS10 ;
    ns1:hasMaterials ns1:M10 ;
    ns1:relatesToHeterostructure ns1:LasingFrequency,
        ns1:OpticalPower,
        ns1:WorkingTemperature .

ns1:HS11 a ns1:LaserHeterostructure ;
    ns1:hasDesignType ns1:LOPhononDepopulation ;
    ns1:hasLayerSequence ns1:LS11 ;
    ns1:hasMaterials ns1:M11 ;
    ns1:relatesToHeterostructure ns1:LasingFrequency,
        ns1:OpticalPower,
        ns1:WorkingTemperature .

ns1:HS12 a ns1:LaserHeterostructure ;
    ns1:hasDesignType ns1:DoubleResonantPhonon ;
    ns1:hasLayerSequence ns1:LS12 ;
    ns1:hasMaterials ns1:M12 ;
    ns1:relatesToHeterostructure ns1:LasingFrequency,
        ns1:OpticalPower,
        ns1:WorkingTemperature .

ns1:HS13 a ns1:LaserHeterostructure .

ns1:HS15 a ns1:LaserHeterostructure .

ns1:HS2 a ns1:LaserHeterostructure ;
    ns1:hasDesignType ns1:DoubleResonantPhonon ;
    ns1:hasLayerSequence ns1:LS2 ;
    ns1:hasMaterials ns1:M2 ;
    ns1:relatesToHeterostructure ns1:LasingFrequency,
        ns1:OpticalPower,
        ns1:WorkingTemperature .

ns1:HS3 a ns1:LaserHeterostructure ;
    ns1:hasDesignType ns1:LOPhononDepopulation ;
    ns1:hasLayerSequence ns1:LS3 ;
    ns1:hasMaterials ns1:M3 ;
    ns1:relatesToHeterostructure ns1:LasingFrequency,
        ns1:OpticalPower,
        ns1:WorkingTemperature .

ns1:HS4 a ns1:LaserHeterostructure ;
    ns1:hasDesignType ns1:DoubleResonantPhonon ;
    ns1:hasLayerSequence ns1:LS4 ;
    ns1:hasMaterials ns1:M4 ;
    ns1:relatesToHeterostructure ns1:LasingFrequency,
        ns1:OpticalPower,
        ns1:WorkingTemperature .

ns1:HS5 a ns1:LaserHeterostructure ;
    ns1:hasDesignType ns1:LOPhononDepopulation ;
    ns1:hasLayerSequence ns1:LS5 ;
    ns1:hasMaterials ns1:M5 ;
    ns1:relatesToHeterostructure ns1:LasingFrequency,
        ns1:OpticalPower,
        ns1:WorkingTemperature .

ns1:HS6 a ns1:LaserHeterostructure ;
    ns1:hasDesignType ns1:BoundToContinum ;
    ns1:hasLayerSequence ns1:LS6 ;
    ns1:hasMaterials ns1:M6 ;
    ns1:relatesToHeterostructure ns1:LasingFrequency,
        ns1:OpticalPower,
        ns1:WorkingTemperature .

ns1:HS8 a ns1:LaserHeterostructure ;
    ns1:hasDesignType ns1:LOPhononDepopulation ;
    ns1:hasLayerSequence ns1:LS8 ;
    ns1:hasMaterials ns1:M8 ;
    ns1:relatesToHeterostructure ns1:LasingFrequency,
        ns1:OpticalPower,
        ns1:WorkingTemperature .

ns1:HS9 a ns1:LaserHeterostructure ;
    ns1:hasDesignType ns1:LOPhononDepopulation ;
    ns1:hasLayerSequence ns1:LS9 ;
    ns1:hasMaterials ns1:M9 ;
    ns1:relatesToHeterostructure ns1:LasingFrequency,
        ns1:OpticalPower,
        ns1:WorkingTemperature .

ns1:LS13 a ns1:LayerSequence ;
    ns1:sequence "3.9/14.0/ 0.6/ 9.1/ 0.6/16.0/ 1.5/12.8/ 1.8/12.2/2.0/12.0/ 2.0/ 11.4/ 2.7/11.3/ 3.5/ 11.6" .

ns1:LS15 a ns1:LayerSequence ;
    ns1:sequence "32.6/79.9/19.0/84.0/29.0/51.6" .

ns1:M13 a ns1:HeterostructureMaterials ;
    ns1:matFormula "GaAs/Al0.15Ga0.85As" .

ns1:M15 a ns1:HeterostructureMaterials ;
    ns1:matFormula "GaAs/Al0.25Ga0.75As" .

ns1:PublicationTitle a owl:DatatypeProperty ;
    rdfs:comment "PublicationTitle represents that an academic article has the publication title in a string."@en ;
    rdfs:domain <http://purl.org/ontology/bibo/AcademicArticle> ;
    rdfs:range xsd:string .

ns1:PublicationYear a owl:DatatypeProperty ;
    rdfs:comment "PublicationYear represents that an academic article has the year of publication in a an integer."@en ;
    rdfs:domain <http://purl.org/ontology/bibo/AcademicArticle> ;
    rdfs:range xsd:integer .

ns1:PublisherName a owl:DatatypeProperty ;
    rdfs:comment "PublisherName represents that an academic article has the publishers name in a string."@en ;
    rdfs:domain <http://purl.org/ontology/bibo/AcademicArticle> ;
    rdfs:range xsd:string .

ns1:QCL1 a ns1:QuantumCascadeLaser ;
    prov:wasAttributedTo <https://www.doi.org/10.1063/1.2189671> ;
    ns1:hasHeterostructure ns1:HS1 ;
    ns1:hasProperty ns1:LasingFrequency,
        ns1:OpticalPower,
        ns1:WorkingTemperature ;
    ns1:hasWorkingMode ns1:ContinousWaveOperation,
        ns1:PulsedOperation .

ns1:QCL10 a ns1:QuantumCascadeLaser .

ns1:QCL11 a ns1:QuantumCascadeLaser .

ns1:QCL12 a ns1:QuantumCascadeLaser .

ns1:QCL13 a ns1:QuantumCascadeLaser .

ns1:QCL14 a ns1:QuantumCascadeLaser ;
    prov:wasAttributedTo <https://www.doi.org/10.1063/1.2216112> ;
    ns1:hasHeterostructure ns1:HS14 ;
    ns1:hasProperty ns1:LasingFrequency,
        ns1:OpticalPower,
        ns1:WorkingTemperature ;
    ns1:hasWorkingMode ns1:ContinousWaveOperation,
        ns1:PulsedOperation .

ns1:QCL15 a ns1:QuantumCascadeLaser .

ns1:QCL2 a ns1:QuantumCascadeLaser .

ns1:QCL3 a ns1:QuantumCascadeLaser .

ns1:QCL4 a ns1:QuantumCascadeLaser .

ns1:QCL5 a ns1:QuantumCascadeLaser .

ns1:QCL6 a ns1:QuantumCascadeLaser .

ns1:QCL7 a ns1:QuantumCascadeLaser ;
    prov:wasAttributedTo <https://www.doi.org/10.1088/0256-307X/30/6/064201> ;
    ns1:hasHeterostructure ns1:HS7 ;
    ns1:hasProperty ns1:LasingFrequency,
        ns1:OpticalPower,
        ns1:WorkingTemperature ;
    ns1:hasWorkingMode ns1:ContinousWaveOperation,
        ns1:PulsedOperation .

ns1:QCL8 a ns1:QuantumCascadeLaser .

ns1:QCL9 a ns1:QuantumCascadeLaser .

ns1:URL a owl:DatatypeProperty ;
    rdfs:comment "URL represents that an academic article has the URL  in a string."@en ;
    rdfs:domain <http://purl.org/ontology/bibo/AcademicArticle> ;
    rdfs:range xsd:string .

ns1:basedOnMaterials a owl:ObjectProperty ;
    rdfs:label "based on materials"@en ;
    rdfs:comment "basedOnMaterials represents that the layer sequence is based on materials in the material composition of a heterostructure."@en ;
    rdfs:domain ns1:LayerSequence ;
    rdfs:range ns1:HeterostructureMaterials .

ns1:composedOf a owl:ObjectProperty ;
    rdfs:label "composed of"@en ;
    rdfs:comment "composedOf represents that materials are composed of atoms."@en ;
    rdfs:domain ns1:HeterostructureMaterials ;
    rdfs:range <https://ftp.ebi.ac.uk/pub/databases/chebi/ontology/#Atom> .

ns1:hasHeterostructure a owl:ObjectProperty ;
    rdfs:label "has heterostructure"@en ;
    rdfs:comment "has heterostructure represents the relationship between a quantum cascade laser and the heterostructural design it has."@en ;
    rdfs:domain ns1:QuantumCascadeLaser ;
    rdfs:range ns1:LaserHeterostructure .

ns1:hasLayerSequence a owl:ObjectProperty ;
    rdfs:label "has layer sequence"@en ;
    rdfs:comment "hasLayerSequence indicates the relationship between a heterostructure and the layer sequence it has."@en ;
    rdfs:domain ns1:LaserHeterostructure ;
    rdfs:range ns1:LayerSequence .

ns1:hasMaterials a owl:ObjectProperty ;
    rdfs:label "has materials"@en ;
    rdfs:comment "hasMaterials represents that a heterostructure has materials that form the heterostructure layer."@en ;
    rdfs:domain ns1:LaserHeterostructure .

ns1:hasProperty a owl:ObjectProperty ;
    rdfs:label "has property"@en ;
    rdfs:comment "hasProperty represents the relationship between a quantum cascade laser device and the property it has."@en ;
    rdfs:domain ns1:QuantumCascadeLaser ;
    rdfs:range mdo-core:Property .

ns1:hasWorkingMode a owl:ObjectProperty ;
    rdfs:label "has working mode"@en ;
    rdfs:comment "hasWorkingMode represents the relationship between a laser device and the working mode in which it is working."@en ;
    rdfs:domain ns1:QuantumCascadeLaser ;
    rdfs:range ns1:LaserWorkingMode .

ns1:matFormula a owl:DatatypeProperty ;
    rdfs:label "material formula"@en ;
    rdfs:comment "matFormula represents that materials have the fomula in a string. The formula indicates the material elemenst used and the number of atoms."@en ;
    rdfs:domain ns1:HeterostructureMaterials ;
    rdfs:range xsd:string .

ns1:relatesToMaterial a owl:ObjectProperty ;
    rdfs:label "relates to material"@en ;
    rdfs:comment "relatesToMaterial refers to the relationship between the heterostructure and the material space it comes from."@en ;
    rdfs:domain ns1:LaserHeterostructure ;
    rdfs:range emmo:Material .

ns1:sequence a owl:DatatypeProperty ;
    rdfs:comment "sequence represents that a layer sequence has a sequence in a string."@en ;
    rdfs:domain ns1:LayerSequence ;
    rdfs:range xsd:string .

<https://opg.optica.org/oe/fulltext.cfm?uri=oe-23-15-19689&id=323020> a <http://purl.org/ontology/bibo/AcademicArticle> ;
    ns1:DOI "10.1364/OE.23.019689 " .

ns4:hasQuantityValue a owl:ObjectProperty ;
    rdfs:label "has quantity value"@en ;
    rdfs:domain ns2:Quantity ;
    rdfs:range ns2:QuantityValue .

ns2:hasQuantityKind a owl:ObjectProperty ;
    rdfs:label "has quantity kind"@en ;
    rdfs:domain ns2:Quantity ;
    rdfs:range ns2:QuantityKind .

ns2:numericValue a owl:DatatypeProperty ;
    rdfs:domain ns2:QuantityValue ;
    rdfs:range xsd:float .

<https://www.doi.org/10.1063/1.1554479> a <http://purl.org/ontology/bibo/AcademicArticle> ;
    ns1:DOI "10.1063/1.1554479" .

<https://www.doi.org/10.1063/1.2737129> a <http://purl.org/ontology/bibo/AcademicArticle> ;
    ns1:DOI "10.1063/1.2737129" .

<https://www.doi.org/10.1063/1.3114418> a <http://purl.org/ontology/bibo/AcademicArticle> ;
    ns1:DOI "10.1063/1.3114418" .

<https://www.doi.org/10.1063/1.4766915> a <http://purl.org/ontology/bibo/AcademicArticle> ;
    ns1:DOI "10.1063/1.4766915" .

<https://www.doi.org/10.1063/1.4862177> a <http://purl.org/ontology/bibo/AcademicArticle> ;
    ns1:DOI "10.1063/1.4862177" .

<https://www.doi.org/10.1063/1.5110305> a <http://purl.org/ontology/bibo/AcademicArticle> ;
    ns1:DOI "10.1063/1.5110305" .

<https://www.doi.org/10.1088/1367-2630/11/12/125022> a <http://purl.org/ontology/bibo/AcademicArticle> ;
    ns1:DOI "10.1088/1367-2630/11/12/125022" .

<https://www.doi.org/10.1088/1367-2630/17/2/023050> a <http://purl.org/ontology/bibo/AcademicArticle> ;
    ns1:DOI "10.1088/1367-2630/17/2/023050" .

<https://www.doi.org/10.1088/1367-2630/18/12/123004> a <http://purl.org/ontology/bibo/AcademicArticle> ;
    ns1:DOI "10.1088/1367-2630/18/12/123004" .

<https://www.doi.org/10.1364/OE.16.003242> a <http://purl.org/ontology/bibo/AcademicArticle> ;
    ns1:DOI "10.1364/OE.16.003242" .

<https://www.doi.org/10.1364/OE.20.003866> a <http://purl.org/ontology/bibo/AcademicArticle> ;
    ns1:DOI "10.1364/OE.20.003866" .

emmo:Material a owl:Class ;
    rdfs:label "EMMO:Material"@en .

<https://ftp.ebi.ac.uk/pub/databases/chebi/ontology/#Atom> a owl:Class ;
    rdfs:label "ChEBI:Atom"@en ;
    rdfs:comment "A chemical entity constituting the smallest component of an element having the chemical properties of the element."@en .

ns1:FrequencyValue a owl:NamedIndividual,
        ns2:QuantityValue ;
    rdfs:label "lasing frequency value"@en ;
    ns3:hasUnit <https://qudt.org/vocab/unit/TeraHZ> ;
    rdfs:comment "Frequency Value refers to the quantity value of the laser lasing frequency."@en ;
    ns2:numericValue "1.9",
        "2.1",
        "2.67",
        "2.83",
        "3",
        "3.2",
        "3.3",
        "3.44",
        "3.9",
        "3.95",
        "4.7",
        "none" .

ns1:HS1 a ns1:LaserHeterostructure ;
    ns1:hasDesignType ns1:LOPhononDepopulation ;
    ns1:hasLayerSequence ns1:LS1 ;
    ns1:hasMaterials ns1:M1 ;
    ns1:relatesToHeterostructure ns1:LasingFrequency,
        ns1:OpticalPower,
        ns1:WorkingTemperature .

ns1:HS14 a ns1:LaserHeterostructure ;
    ns1:hasDesignType ns1:LOPhononDepopulation ;
    ns1:hasLayerSequence ns1:LS14 ;
    ns1:hasMaterials ns1:M14 ;
    ns1:relatesToHeterostructure ns1:LasingFrequency,
        ns1:OpticalPower,
        ns1:WorkingTemperature .

ns1:HS7 a ns1:LaserHeterostructure ;
    ns1:hasDesignType ns1:BoundToContinum ;
    ns1:hasLayerSequence ns1:LS7 ;
    ns1:hasMaterials ns1:M7 ;
    ns1:relatesToHeterostructure ns1:LasingFrequency,
        ns1:OpticalPower,
        ns1:WorkingTemperature .

ns1:LS1 a ns1:LayerSequence ;
    ns3:hasUnit <https://qudt.org/vocab/unit/ANGSTROM> ;
    ns1:basedOnMaterials ns1:M1 ;
    ns1:sequence "49/78/23/76/32/76/52/168" .

ns1:LS10 a ns1:LayerSequence ;
    ns3:hasUnit <https://qudt.org/vocab/unit/ANGSTROM> ;
    ns1:basedOnMaterials ns1:M10 ;
    ns1:sequence "217 /43 /111 /35 /132 /20/128 /51" .

ns1:LS11 a ns1:LayerSequence ;
    ns3:hasUnit <https://qudt.org/vocab/unit/ANGSTROM> ;
    ns1:basedOnMaterials ns1:M11 ;
    ns1:sequence "43/89/24.6/81.5/41/160" .

ns1:LS12 a ns1:LayerSequence ;
    ns3:hasUnit <https://qudt.org/vocab/unit/ANGSTROM> ;
    ns1:basedOnMaterials ns1:M12 ;
    ns1:sequence "9/79/25/66/41/156/33/90" .

ns1:LS14 a ns1:LayerSequence ;
    ns3:hasUnit <https://qudt.org/vocab/unit/ANGSTROM> ;
    ns1:basedOnMaterials ns1:M14 ;
    ns1:sequence "31/93/14/82/23/175/11/105/14/85/20/175/17/105" .

ns1:LS2 a ns1:LayerSequence ;
    ns3:hasUnit <https://qudt.org/vocab/unit/NanoM> ;
    ns1:basedOnMaterials ns1:M2 ;
    ns1:sequence "4.24/8.48/3.11/11.02/2.54/7.91/4.24/16.67" .

ns1:LS3 a ns1:LayerSequence ;
    ns3:hasUnit <https://qudt.org/vocab/unit/ANGSTROM> ;
    ns1:basedOnMaterials ns1:M3 ;
    ns1:sequence "54/78/24/64/38/148/24/94" .

ns1:LS4 a ns1:LayerSequence ;
    ns3:hasUnit <https://qudt.org/vocab/unit/NanoM> ;
    ns1:basedOnMaterials ns1:M4 ;
    ns1:sequence "4.8/8.5/2.8/8.5/4.2/16.4" .

ns1:LS5 a ns1:LayerSequence ;
    ns3:hasUnit <https://qudt.org/vocab/unit/ANGSTROM> ;
    ns1:basedOnMaterials ns1:M5 ;
    ns1:sequence "35/48/8/38.9/9/72/2/85.6/5/66" .

ns1:LS6 a ns1:LayerSequence ;
    ns3:hasUnit <https://qudt.org/vocab/unit/NanoM> ;
    ns1:basedOnMaterials ns1:M6 ;
    ns1:sequence "5.5/11.0/1.8/11.5/3.8/9.4/4.2/18.4" .

ns1:LS7 a ns1:LayerSequence ;
    ns3:hasUnit <https://qudt.org/vocab/unit/NanoM> ;
    ns1:basedOnMaterials ns1:M7 ;
    ns1:sequence "4.0/12/0.5/22.3/0.8/21.5/0.9/17.8/1/14.5/1.3/13.2?/2.2/13.4/2.8/17" .

ns1:LS8 a ns1:LayerSequence ;
    ns3:hasUnit <https://qudt.org/vocab/unit/NanoM> ;
    ns1:basedOnMaterials ns1:M8 ;
    ns1:sequence "5.1/9.3/1.0/10.5/3.3/8.7/4.2/16.5" .

ns1:LS9 a ns1:LayerSequence ;
    ns3:hasUnit <https://qudt.org/vocab/unit/NanoM> ;
    ns1:basedOnMaterials ns1:M9 ;
    ns1:sequence "2.0/20.3/2.0/3.0/14.4/1.0/13.5/3.0" .

ns1:PowerValue a owl:NamedIndividual,
        ns2:QuantityValue ;
    rdfs:label "power value"@en ;
    ns3:hasUnit <https://qudt.org/vocab/unit/MilliW> ;
    rdfs:comment "PowerValue refers to the quanity value of the laser optical power."@en ;
    ns2:numericValue "10",
        "100",
        "2.5",
        "200",
        "38",
        "62",
        "9",
        "none" .

ns1:WorkingTempValue a owl:NamedIndividual,
        ns2:QuantityValue ;
    rdfs:label "working temperature value"@en ;
    ns3:hasUnit <https://qudt.org/vocab/unit/K> ;
    rdfs:comment "WorkingTempValue refers to the quantity value of the laser working/operation temperature."@en ;
    ns2:numericValue "100",
        "105",
        "110",
        "138",
        "142",
        "144",
        "150",
        "151",
        "178",
        "186",
        "195",
        "200",
        "210.5",
        "45",
        "60",
        "65",
        "85",
        "95",
        "none" .

<https://qudt.org/vocab/quantitykind/Frequency> a ns2:QuantityKind .

<https://qudt.org/vocab/quantitykind/Power> a ns2:QuantityKind .

<https://qudt.org/vocab/quantitykind/Temperature> a ns2:QuantityKind .

<https://qudt.org/vocab/unit/K> a ns2:Unit .

<https://qudt.org/vocab/unit/MilliW> a ns2:Unit .

<https://qudt.org/vocab/unit/TeraHZ> a ns2:Unit .

<https://www.doi.org/10.1063/1.2189671> a <http://purl.org/ontology/bibo/AcademicArticle> ;
    ns1:DOI "10.1063/1.2189671" .

<https://www.doi.org/10.1063/1.2216112> a <http://purl.org/ontology/bibo/AcademicArticle> ;
    ns1:DOI "10.1063/1.2216112" .

<https://www.doi.org/10.1088/0256-307X/30/6/064201> a <http://purl.org/ontology/bibo/AcademicArticle> ;
    ns1:DOI "10.1088/0256-307X/30/6/064201" .

<https://www.w3.org/TR/prov-o/#Agent> a owl:Class ;
    rdfs:comment "An agent is something that bears some form of responsibility for an activity taking place, for the existence of an entity, or for another agent's activity."@en .

ns1:M1 a ns1:HeterostructureMaterials ;
    ns1:matFormula "GaAs/Al0.15Ga0.85As" .

ns1:M10 a ns1:HeterostructureMaterials ;
    ns1:matFormula "In 0.53 Ga 0.47 As/Al 0.17In 0.52 Ga 0.31 As" .

ns1:M11 a ns1:HeterostructureMaterials ;
    ns1:matFormula "GaAs/Al0.15Ga0.85As" .

ns1:M12 a ns1:HeterostructureMaterials ;
    ns1:matFormula "GaAs/Al0.15Ga0.85As" .

ns1:M14 a ns1:HeterostructureMaterials ;
    ns1:matFormula "GaAs/Al0.3Ga0.7As" .

ns1:M2 a ns1:HeterostructureMaterials ;
    ns1:matFormula "GaAs/Al0.15Ga0.85As" .

ns1:M3 a ns1:HeterostructureMaterials ;
    ns1:matFormula "GaAs/Al0.15Ga0.85As" .

ns1:M4 a ns1:HeterostructureMaterials ;
    ns1:matFormula "GaAs/Al0.15Ga0.85As" .

ns1:M5 a ns1:HeterostructureMaterials ;
    ns1:matFormula "GaAs/Al0.25Ga0.75As" .

ns1:M6 a ns1:HeterostructureMaterials ;
    ns1:matFormula "GaAs/Al0.15Ga0.85As" .

ns1:M7 a ns1:HeterostructureMaterials ;
    ns1:matFormula "GaAs/Al0.15Ga0.85As" .

ns1:M8 a ns1:HeterostructureMaterials ;
    ns1:matFormula "GaAs/Al0.15Ga0.85As" .

ns1:M9 a ns1:HeterostructureMaterials ;
    ns1:matFormula "In0.53Ga0.47As/GaAs0.51Sb0.49" .

ns1:correspondsToWorkingMode a owl:ObjectProperty ;
    rdfs:label "corresponds to working mode"@en ;
    rdfs:comment "correspondsToWorkingMode represents the relationship between a property and the laser working mode under which it was obtained."@en ;
    rdfs:domain mdo-core:Property ;
    rdfs:range ns1:LaserWorkingMode .

ns1:hasDesignType a owl:ObjectProperty ;
    rdfs:label "has design type"@en ;
    rdfs:comment "hasDesignType indicates the relatioship between the laser heterostructure and the desgn type on whch it is based."@en ;
    rdfs:domain ns1:LaserHeterostructure ;
    rdfs:range ns1:LaserDesignType .

ns1:BoundToContinum a owl:NamedIndividual,
        ns1:LaserDesignType ;
    rdfs:label "bound to continum"@en ;
    rdfs:comment "A laser design where the sequence of material in the active region is made with more or less increasing width of layers in the multistack of material."@en .

ns1:DoubleResonantPhonon a owl:NamedIndividual,
        ns1:LaserDesignType ;
    rdfs:label "double resonant phonon"@en ;
    rdfs:comment "A laser design where two quantum well are resonant."@en .

ns2:Quantity a owl:Class ;
    rdfs:comment "A quantity is the measurement of an observable property of a particular object, event, or physical system."@en .

ns1:ContinousWaveOperation a owl:NamedIndividual,
        ns1:LaserWorkingMode ;
    rdfs:label "continous wave operation"@en ;
    rdfs:comment "Continous Wave Operation refers to the laser operation mode in which laser beams are emitted continously."@en .

ns1:PulsedOperation a owl:NamedIndividual,
        ns1:LaserWorkingMode ;
    rdfs:label "pulsed operation"@en ;
    rdfs:comment "Pulse operation  refers to the laser operation mode in which laser beams are emitted in pulses."@en .

ns2:QuantityKind a owl:Class ;
    rdfs:label "Quantity Kind"@en ;
    rdfs:comment "A Quantity Kind is any observable property that can be measured and quantified numerically. Familiar examples include physical properties such as length, mass, time, force, energy, power, electric charge, etc."@en .

ns2:Unit a owl:Class ;
    rdfs:label "Unit"@en ;
    rdfs:comment "A unit of measure, or unit, is a particular quantity value that has been chosen as a scale for measuring other quantities the same kind (more generally of equivalent dimension)."@en .

mdo-core:Property a owl:Class ;
    rdfs:label "Property"@en ;
    rdfs:comment "A property in materials design is data pertaining to at least one material or materials system, representing a quantifiable aspect of one material or materials system."@en ;
    rdfs:subClassOf [ a owl:Class ;
            owl:intersectionOf ( [ a owl:Restriction ;
                        owl:allValuesFrom ns1:LaserWorkingMode ;
                        owl:onProperty ns1:correspondsToWorkingMode ] [ a owl:Restriction ;
                        owl:onClass ns1:LaserWorkingMode ;
                        owl:onProperty ns1:correspondsToWorkingMode ;
                        owl:qualifiedCardinality "1"^^xsd:nonNegativeInteger ] ) ],
        ns2:Quantity .

ns1:LaserDesignType a owl:Class ;
    rdfs:label "Laser Design Type"@en ;
    rdfs:comment "Represents the geometrical aspects of the laser design."@en .

ns1:LaserWorkingMode a owl:Class ;
    rdfs:label "Laser Working Mode"@en ;
    rdfs:comment "Refers to the nature in which the laser beams are emmitted."@en .

ns2:QuantityValue a owl:Class ;
    rdfs:label "Quantity Value"@en .

<https://qudt.org/vocab/unit/NanoM> a ns2:Unit .

ns1:LOPhononDepopulation a owl:NamedIndividual,
        ns1:LaserDesignType ;
    rdfs:label "LO Phonon Depopulation"@en ;
    rdfs:comment "LO Phonon depopulation refers to the laser design where the sequence of material in the active region is designed to provide laser effect from longitudinal Optical Phonons."@en .

ns1:LasingFrequency a owl:NamedIndividual,
        mdo-core:Property ;
    rdfs:label "lasing frequency"@en ;
    rdfs:comment "LasingFrequency refers to the frequency at which the quantum cascade lasers emits the laser beams."@en ;
    ns4:hasQuantityValue ns1:FrequencyValue ;
    ns2:hasQuantityKind <https://qudt.org/vocab/quantitykind/Frequency> .

ns1:OpticalPower a owl:NamedIndividual,
        mdo-core:Property ;
    rdfs:label "optical power"@en ;
    rdfs:comment "OpticalPower refers to the laser output power."@en ;
    ns4:hasQuantityValue ns1:PowerValue ;
    ns2:hasQuantityKind <https://qudt.org/vocab/quantitykind/Power> .

ns1:WorkingTemperature a owl:NamedIndividual,
        mdo-core:Property ;
    rdfs:label "working temperature"@en ;
    rdfs:comment "WorkingTemperature refers to the operation temperature under which the quantum cascade laser emmits the laser beams."@en ;
    ns1:correspondsToWorkingMode ns1:ContinousWaveOperation,
        ns1:PulsedOperation ;
    ns4:hasQuantityValue ns1:WorkingTempValue ;
    ns2:hasQuantityKind <https://qudt.org/vocab/quantitykind/Temperature> .

ns1:HeterostructureMaterials a owl:Class ;
    rdfs:label "Heterostructure Materials"@en ;
    rdfs:comment "Heterostructure Materials refers to the materials forming the heterostructure layer."@en .

ns1:LayerSequence a owl:Class ;
    rdfs:label "Layer Sequence"@en ;
    rdfs:comment "Reprsents the sequence and thickness of materials composing the heterostructure."@en .

ns1:QuantumCascadeLaser a owl:Class ;
    rdfs:label "Quantum Cascade Laser"@en ;
    rdfs:comment "Semiconductor lasers that operate in the mid to far-infrared region."@en .

ns1:LaserHeterostructure a owl:Class ;
    rdfs:label "Laser Heterostructure"@en ;
    rdfs:comment "A layered material composed of different semiconductor materials."@en ;
    rdfs:subClassOf [ a owl:Class ;
            owl:intersectionOf ( [ a owl:Restriction ;
                        owl:allValuesFrom ns1:LaserDesignType ;
                        owl:onProperty ns1:hasDesignType ] [ a owl:Restriction ;
                        owl:onClass ns1:LaserDesignType ;
                        owl:onProperty ns1:hasDesignType ;
                        owl:qualifiedCardinality "1"^^xsd:nonNegativeInteger ] ) ] .

<http://purl.org/ontology/bibo/AcademicArticle> a owl:Class ;
    rdfs:label "Academic Article"@en ;
    rdfs:comment "A scholarly academic article, typically published in a journal."@en ;
    rdfs:subClassOf <https://www.w3.org/TR/prov-o/#Agent> .

