<?xml version="1.0" encoding="UTF-8"?>
<rdf:RDF xmlns="https://github.com/DeperiasKerre/qcl_Onto/tree/main/qclontology/"
     xml:base="https://github.com/DeperiasKerre/qcl_Onto/tree/main/qclontology/"
     xmlns:owl="http://www.w3.org/2002/07/owl#"
     xmlns:rdf="http://www.w3.org/1999/02/22-rdf-syntax-ns#"
     xmlns:xml="http://www.w3.org/XML/1998/namespace"
     xmlns:xsd="http://www.w3.org/2001/XMLSchema#"
     xmlns:emmo="http://emmo.info/domains/emmo-material.owl#"
     xmlns:qudt="http://qudt.org/schema/qudt/"
     xmlns:rdfs="http://www.w3.org/2000/01/rdf-schema#"
     xmlns:vann="http://purl.org/vocab/vann/"
     xmlns:dcterms="http://purl.org/dc/terms/"
     xmlns:qudt-unit="http://qudt.org/vocab/unit/">

     <!--Ontology Metadata-->

     <owl:Ontology rdf:about="https://github.com/DeperiasKerre/qcl_Onto/">
          <owl:versionIRI rdf:resource="https://github.com/DeperiasKerre/qcl_Onto/tree/main/qclontology"/>
          <dcterms:contributor rdf:datatype="http://www.w3.org/2001/XMLSchema#string">Anne Laurent</dcterms:contributor>
          <dcterms:contributor rdf:datatype="http://www.w3.org/2001/XMLSchema#string">Kenneth Maussang</dcterms:contributor>
          <dcterms:contributor rdf:datatype="http://www.w3.org/2001/XMLSchema#string">Dickson Owuor</dcterms:contributor>
          <dcterms:created>2023-09-27</dcterms:created>
          <dcterms:creator rdf:datatype="http://www.w3.org/2001/XMLSchema#string">Deperias Kerre</dcterms:creator>
          <dcterms:license>https://github.com/DeperiasKerre/qcl_Onto/blob/main/LICENSE</dcterms:license>
          <dcterms:title xml:lang="en">An Ontological Representation of the Quantum Cascade Laser Properties</dcterms:title>
        <vann:preferredNamespacePrefix>qclontology</vann:preferredNamespacePrefix>
        <vann:preferredNamespaceUri>https://github.com/DeperiasKerre/qcl_Onto/tree/main/qclontology/</vann:preferredNamespaceUri>
        <rdfs:comment xml:lang="en">This is an ontological representation of the quantum cascade laser properties.</rdfs:comment>
        <rdfs:seeAlso>https://github.com/DeperiasKerre/qcl_Onto</rdfs:seeAlso>
        <owl:versionInfo rdf:datatype="http://www.w3.org/2001/XMLSchema#string">1.0</owl:versionInfo>
     </owl:Ontology>

     <!--Annotation properties-->

     <!--contributor -->

    <owl:AnnotationProperty rdf:about="http://purl.org/dc/terms/contributor"/>
    


    <!--created -->

    <owl:AnnotationProperty rdf:about="http://purl.org/dc/terms/created"/>
    


    <!--creator -->

    <owl:AnnotationProperty rdf:about="http://purl.org/dc/terms/creator"/>
    


    <!--license -->

    <owl:AnnotationProperty rdf:about="http://purl.org/dc/terms/license"/>
    


    <!--title -->

    <owl:AnnotationProperty rdf:about="http://purl.org/dc/terms/title"/>
    


    <!--preferredNamespacePrefix -->

    <owl:AnnotationProperty rdf:about="http://purl.org/vocab/vann/preferredNamespacePrefix"/>
    


    <!--preferredNamespaceUri -->

    <owl:AnnotationProperty rdf:about="http://purl.org/vocab/vann/preferredNamespaceUri"/>

 
    <!--Datatypes-->

    <!--string-->
    <rdfs:Datatype rdf:about="http://www.w3.org/2001/XMLSchema#string"/>
    
    <!--Integer-->
    <rdfs:Datatype rdf:about="http://www.w3.org/2001/XMLSchema#integer"/>
 
    <!--Double-->
    <rdfs:Datatype rdf:about="http://www.w3.org/2001/XMLSchema#double"/>

    <!--Object Properties-->

    <!--hasHeterostructure-->

    <owl:ObjectProperty rdf:about="https://github.com/DeperiasKerre/qcl_Onto/blob/main/qclontology/qclontov1.owl#hasHeterostructure">
        <rdfs:domain rdf:resource="https://github.com/DeperiasKerre/qcl_Onto/blob/main/qclontology/qclontov1.owl#QuantumCascadeLaser"/>
        <rdfs:range rdf:resource="https://github.com/DeperiasKerre/qcl_Onto/blob/main/qclontology/qclontov1.owl#Heterostructure"/>
        <rdfs:comment xml:lang="en">hasHeterostructure represents the relationship between a quantum cascade laser device and the corresponding heterostructure it has.</rdfs:comment>
        <rdfs:label xml:lang="en">has heterostructure</rdfs:label>
    </owl:ObjectProperty>

    <!--hasWorkingMode-->

    <owl:ObjectProperty rdf:about="https://github.com/DeperiasKerre/qcl_Onto/blob/main/qclontology/qclontov1.owl#hasWorkingMode">
        <rdfs:domain rdf:resource="https://github.com/DeperiasKerre/qcl_Onto/blob/main/qclontology/qclontov1.owl#QuantumCascadeLaser"/>
        <rdfs:range rdf:resource="https://github.com/DeperiasKerre/qcl_Onto/blob/main/qclontology/qclontov1.owl#LaserWorkingMode"/>
        <rdfs:comment xml:lang="en">hasWorkingMode represents the relationship between a quantum cascade laser device and the corresponding laser working mode it has.</rdfs:comment>
        <rdfs:label xml:lang="en">has working mode</rdfs:label>
    </owl:ObjectProperty>

    <!--hasPhysicalProperty-->

    <owl:ObjectProperty rdf:about="https://github.com/DeperiasKerre/qcl_Onto/blob/main/qclontology/qclontov1.owl#hasPhysicalProperty">
        <rdfs:domain rdf:resource="https://github.com/DeperiasKerre/qcl_Onto/blob/main/qclontology/qclontov1.owl#QuantumCascadeLaser"/>
        <rdfs:range rdf:resource="https://w3id.org/mdo/core/PhysicalProperty"/>
        <rdfs:comment xml:lang="en">hasPhysicalProperty represents the relationship that a quantum cascade laser has a physical property</rdfs:comment>
        <rdfs:label xml:lang="en">has physical property</rdfs:label>
    </owl:ObjectProperty>

    <!--hasQuantityKind -->

    <owl:ObjectProperty rdf:about="http://qudt.org/schema/qudt/hasQuantityKind">
        <rdfs:domain rdf:resource="http://qudt.org/schema/qudt/Quantity"/>
        <rdfs:range rdf:resource="http://qudt.org/schema/qudt/QuantityKind"/>
        <rdfs:comment xml:lang="en">hasQuantityKind represents that Quanity has a QuantityKind </rdfs:comment>
    </owl:ObjectProperty>

    <!--relatesToMaterial-->

    <owl:ObjectProperty rdf:about="https://github.com/DeperiasKerre/qcl_Onto/blob/main/qclontology/qclontov1.owl#relatesToMaterial">
        <rdfs:domain rdf:resource="https://github.com/DeperiasKerre/qcl_Onto/blob/main/qclontology/qclontov1.owl#Heterostructure"/>
        <rdfs:range rdf:resource="http://emmo.info/domains/emmo-material.owl#EMMO_4207e895_8b83_4318_996a_72cfb32acd94"/>
        <rdfs:comment xml:lang="en">relatesToMaterial represents the relationship between a heterostructure and the materials it comes from.</rdfs:comment>
        <rdfs:label xml:lang="en">relates to material</rdfs:label>
    </owl:ObjectProperty>

    <!--hasDesignType-->

    <owl:ObjectProperty rdf:about="https://github.com/DeperiasKerre/qcl_Onto/blob/main/qclontology/qclontov1.owl#hasDesignType">
        <rdfs:domain rdf:resource="https://github.com/DeperiasKerre/qcl_Onto/blob/main/qclontology/qclontov1.owl#Heterostructure"/>
        <rdfs:range rdf:resource="https://github.com/DeperiasKerre/qcl_Onto/blob/main/qclontology/qclontov1.owl#LaserDesignType"/>
        <rdfs:comment xml:lang="en">hasDesignType represents the relationship between a heterostructure and the corresponding laser design type it has.</rdfs:comment>
        <rdfs:label xml:lang="en">has design type</rdfs:label>
    </owl:ObjectProperty>

    <!--hasMaterialComposition-->

    <owl:ObjectProperty rdf:about="https://github.com/DeperiasKerre/qcl_Onto/blob/main/qclontology/qclontov1.owl#hasMaterialComposition">
        <rdfs:domain rdf:resource="https://github.com/DeperiasKerre/qcl_Onto/blob/main/qclontology/qclontov1.owl#Heterostructure"/>
        <rdfs:range rdf:resource="https://github.com/DeperiasKerre/qcl_Onto/blob/main/qclontology/qclontov1.owl#MaterialComposition"/>
        <rdfs:comment xml:lang="en">hasMaterialComposition represents the relationship between a heterostructure and the semiconductor materials it has.</rdfs:comment>
        <rdfs:label xml:lang="en">has material composition</rdfs:label>
    </owl:ObjectProperty>

    <!--relatesToHeterostructure-->

    <owl:ObjectProperty rdf:about="https://github.com/DeperiasKerre/qcl_Onto/blob/main/qclontology/qclontov1.owl#relatesToHeterostructure">
        <rdfs:domain rdf:resource="https://w3id.org/mdo/core/PhysicalProperty"/>
        <rdfs:range rdf:resource="https://github.com/DeperiasKerre/qcl_Onto/blob/main/qclontology/qclontov1.owl#Heterostructure"/>
        <rdfs:comment xml:lang="en">relatesToHeterostructure represents the relationship between a physical property and the heterostructure it correspond to.</rdfs:comment>
        <rdfs:label xml:lang="en">relates to heterostructure</rdfs:label>
    </owl:ObjectProperty>

    <!--correspondsToWorkingMode-->

    <owl:ObjectProperty rdf:about="https://github.com/DeperiasKerre/qcl_Onto/blob/main/qclontology/qclontov1.owl#correspondsToWorkingMode">
        <rdfs:domain rdf:resource="https://w3id.org/mdo/core/PhysicalProperty"/>
        <rdfs:range rdf:resource="https://github.com/DeperiasKerre/qcl_Onto/blob/main/qclontology/qclontov1.owl#LaserWorkingMode"/>
        <rdfs:comment xml:lang="en">correspondsToWorkingMode represents the relationship between a physical property and the laser working mode under which it was obtained .</rdfs:comment>
        <rdfs:label xml:lang="en">corresponds to working mode</rdfs:label>
    </owl:ObjectProperty>

    <!--quantityValue-->

    <owl:ObjectProperty rdf:about="http://qudt.org/schema/qudt/quantityValue">
        <rdfs:domain rdf:resource="http://qudt.org/schema/qudt/Quantity"/>
        <rdfs:range rdf:resource="http://qudt.org/schema/qudt/QuantityValue"/>
        <rdfs:comment xml:lang="en">QuantityValue represents that Quanity has a QuantityValue</rdfs:comment>
    </owl:ObjectProperty>

    <!--unit-->

    <owl:ObjectProperty rdf:about="http://qudt.org/schema/qudt/unit">
        <rdfs:domain rdf:resource="http://qudt.org/schema/qudt/QuantityValue"/>
        <rdfs:range rdf:resource="http://qudt.org/schema/qudt/Unit"/>
         <rdfs:comment xml:lang="en">A reference to the unit of measure of a quantity (variable or constant) of interest.</rdfs:comment>
    </owl:ObjectProperty>

    <!-- http://www.w3.org/ns/prov#wasAttributedTo -->

    <owl:ObjectProperty rdf:about="http://www.w3.org/ns/prov#wasAttributedTo">
        <rdfs:domain rdf:resource="https://github.com/DeperiasKerre/qcl_Onto/blob/main/qclontology/qclontov1.owl#Heterostructure"/>
        <rdfs:range rdf:resource="https://github.com/DeperiasKerre/qcl_Onto/blob/main/qclontology/qclontov1.owl#ReferenceInfoAgent"/>
         <rdfs:comment xml:lang="en">A reference to the scientific article documenting the heterostructure.</rdfs:comment>
    </owl:ObjectProperty>

    <!-- http://www.w3.org/ns/prov#wasAttributedTo -->

    <owl:ObjectProperty rdf:about="http://www.w3.org/ns/prov#wasAttributedTo">
        <rdfs:domain rdf:resource="https://w3id.org/mdo/core/PhysicalProperty"/>
        <rdfs:range rdf:resource="https://github.com/DeperiasKerre/qcl_Onto/blob/main/qclontology/qclontov1.owl#ReferenceInfoAgent"/>
         <rdfs:comment xml:lang="en">A reference to the scientific article documenting the physical property.</rdfs:comment>
    </owl:ObjectProperty>

    <!--Data Properties-->

    <!--WorkingModeName-->

    <owl:DatatypeProperty rdf:about="https://github.com/DeperiasKerre/qcl_Onto/blob/main/qclontology/qclontov1.owl#WorkingModeName">
        <rdfs:domain rdf:resource="https://github.com/DeperiasKerre/qcl_Onto/blob/main/qclontology/qclontov1.owl#LaserWorkingMode"/>
        <rdfs:range rdf:resource="http://www.w3.org/2001/XMLSchema#string"/>
        <rdfs:comment xml:lang="en">WorkingModeName represents that the quantum cascade laser working mode has the name in a string.</rdfs:comment>
        <rdfs:label xml:lang="en">working mode name</rdfs:label>
    </owl:DatatypeProperty>
  
    <!--PropertyName -->

    <owl:DatatypeProperty rdf:about="https://w3id.org/mdo/core/PropertyName">
        <rdfs:domain rdf:resource="https://w3id.org/mdo/core/Property"/>
        <rdfs:range rdf:resource="http://www.w3.org/2001/XMLSchema#string"/>
        <rdfs:comment xml:lang="en">PropertyName represents that a property has the name in a string.</rdfs:comment>
        <rdfs:label xml:lang="en">property name</rdfs:label>
    </owl:DatatypeProperty>

    <!--DesignTypeName-->

    <owl:DatatypeProperty rdf:about="https://github.com/DeperiasKerre/qcl_Onto/blob/main/qclontology/qclontov1.owl#DesignTypeName">
        <rdfs:domain rdf:resource="https://github.com/DeperiasKerre/qcl_Onto/blob/main/qclontology/qclontov1.owl#LaserDesignType"/>
        <rdfs:range rdf:resource="http://www.w3.org/2001/XMLSchema#string"/>
        <rdfs:comment xml:lang="en">DesignTypeName represents that the quantum cascade laser Design Type has the name in a string.</rdfs:comment>
        <rdfs:label xml:lang="en">working mode name</rdfs:label>
    </owl:DatatypeProperty>

    <!--formula-->

    <owl:DatatypeProperty rdf:about="https://github.com/DeperiasKerre/qcl_Onto/blob/main/qclontology/qclontov1.owl#formula">
        <rdfs:domain rdf:resource="https://github.com/DeperiasKerre/qcl_Onto/blob/main/qclontology/qclontov1.owl#MaterialComposition"/>
        <rdfs:range rdf:resource="http://www.w3.org/2001/XMLSchema#string"/>
        <rdfs:comment xml:lang="en">formula represents that the heterostructure material composition has a formula in a string.</rdfs:comment>
        <rdfs:label xml:lang="en">formula</rdfs:label>
    </owl:DatatypeProperty>

    <!--numericalValue -->

    <owl:DatatypeProperty rdf:about="http://qudt.org/schema/qudt/numericalValue">
        <rdfs:domain rdf:resource="http://qudt.org/schema/qudt/QuantityValue"/>
        <rdfs:range rdf:resource="http://www.w3.org/2001/XMLSchema#double"/>
    </owl:DatatypeProperty>

    <!--AuthorName -->

    <owl:DatatypeProperty rdf:about="https://github.com/DeperiasKerre/qcl_Onto/blob/main/qclontology/qclontov1.owl#AuthorName">
        <rdfs:domain rdf:resource="https://github.com/DeperiasKerre/qcl_Onto/blob/main/qclontology/qclontov1.owl#ReferenceInfoAgent"/>
        <rdfs:range rdf:resource="http://www.w3.org/2001/XMLSchema#string"/>
        <rdfs:comment xml:lang="en">AuthorName represents that a reference info agent (scientific article) has the author&apos;s name in a string.</rdfs:comment>
        <rdfs:label xml:lang="en">author name</rdfs:label>
    </owl:DatatypeProperty>

    <!--DOI-->

    <owl:DatatypeProperty rdf:about="https://github.com/DeperiasKerre/qcl_Onto/blob/main/qclontology/qclontov1.owl#DOI">
        <rdfs:domain rdf:resource="https://github.com/DeperiasKerre/qcl_Onto/blob/main/qclontology/qclontov1.owl#ReferenceInfoAgent"/>
        <rdfs:range rdf:resource="http://www.w3.org/2001/XMLSchema#string"/>
        <rdfs:comment xml:lang="en">DOI represents that a reference info agent has the DOI in a string.</rdfs:comment>
        <rdfs:label xml:lang="en">DOI</rdfs:label>
    </owl:DatatypeProperty>
    
    <!--PublisherName -->

    <owl:DatatypeProperty rdf:about="https://github.com/DeperiasKerre/qcl_Onto/blob/main/qclontology/qclontov1.owl#PublisherName">
        <rdfs:domain rdf:resource="https://github.com/DeperiasKerre/qcl_Onto/blob/main/qclontology/qclontov1.owl#ReferenceInfoAgent"/>
        <rdfs:range rdf:resource="http://www.w3.org/2001/XMLSchema#string"/>
        <rdfs:comment xml:lang="en">PublisherName represents that a reference info agent has the publisher&apos;s name in a string.</rdfs:comment>
        <rdfs:label xml:lang="en">publisher name</rdfs:label>
    </owl:DatatypeProperty>

    <!--PublicationYear-->

    <owl:DatatypeProperty rdf:about="https://github.com/DeperiasKerre/qcl_Onto/blob/main/qclontology/qclontov1.owl#PublisherYear">
        <rdfs:domain rdf:resource="https://github.com/DeperiasKerre/qcl_Onto/blob/main/qclontology/qclontov1.owl#ReferenceInfoAgent"/>
        <rdfs:range rdf:resource="http://www.w3.org/2001/XMLSchema#integer"/>
        <rdfs:comment xml:lang="en">PublicationYear represents that a reference info agent has the year in which it was published in an integer.</rdfs:comment>
        <rdfs:label xml:lang="en">publication year</rdfs:label>
    </owl:DatatypeProperty>

    <!--PublicationTitle-->

    <owl:DatatypeProperty rdf:about="https://github.com/DeperiasKerre/qcl_Onto/blob/main/qclontology/qclontov1.owl#PublicationTitle">
        <rdfs:domain rdf:resource="https://github.com/DeperiasKerre/qcl_Onto/blob/main/qclontology/qclontov1.owl#ReferenceInfoAgent"/>
        <rdfs:range rdf:resource="http://www.w3.org/2001/XMLSchema#string"/>
        <rdfs:comment xml:lang="en">PublicationTitle represents that a reference info agent has the publication&apos;s title in a string.</rdfs:comment>
        <rdfs:label xml:lang="en">publication title</rdfs:label>
    </owl:DatatypeProperty>
    

    <!--PublicationURL -->

    <owl:DatatypeProperty rdf:about="https://github.com/DeperiasKerre/qcl_Onto/blob/main/qclontology/qclontov1.owl#PublicationURL">
        <rdfs:domain rdf:resource="https://github.com/DeperiasKerre/qcl_Onto/blob/main/qclontology/qclontov1.owl#ReferenceInfoAgent"/>
        <rdfs:range rdf:resource="http://www.w3.org/2001/XMLSchema#string"/>
        <rdfs:comment xml:lang="en">PublicationURL represents that a reference info agent has the URL to the publication in a string.</rdfs:comment>
        <rdfs:label xml:lang="en">publication URL</rdfs:label>
    </owl:DatatypeProperty>
    
    <!--Classes-->
  
    <!--Owl Thing Class-->

    <owl:Class rdf:about="http://www.w3.org/2002/07/owl#Thing">
         <!--rdfs:label xml:lang="en">Thing</rdfs:label-->
         <rdfs:comment xml:lang="en">The class of OWL individuals.</rdfs:comment>
    </owl:Class>

    <!--Quantity Class-->

    <owl:Class rdf:about="http://qudt.org/schema/qudt/Quantity">
         <rdfs:subClassOf rdf:resource="http://www.w3.org/2002/07/owl#Thing"/>
         <rdfs:label xml:lang="en">Quantity</rdfs:label>
         <rdfs:comment xml:lang="en">A quantity is the measurement of an observable property of a particular object, event, or physical system.</rdfs:comment>
    </owl:Class>

    <!--Quantum Casacde Laser-->

    <owl:Class rdf:about="https://github.com/DeperiasKerre/qcl_Onto/blob/main/qclontology/qclontov1.owl#QuantumCascadeLaser">
         <rdfs:subClassOf rdf:resource="http://www.w3.org/2002/07/owl#Thing"/>
         <rdfs:label xml:lang="en">Quantum Cascade Laser</rdfs:label>
         <rdfs:comment xml:lang="en">Semiconductor lasers that operate in the mid-to-far infrared region.</rdfs:comment>
    </owl:Class>

    <!--Heterostructure-->

    <owl:Class rdf:about="https://github.com/DeperiasKerre/qcl_Onto/blob/main/qclontology/qclontov1.owl#Heterostructure">
         <rdfs:subClassOf>
            <owl:Restriction>
                <owl:onProperty rdf:resource="https://github.com/DeperiasKerre/qcl_Onto/blob/main/qclontology/qclontov1.owl#hasDesignType"/>
                <owl:qualifiedCardinality rdf:datatype="http://www.w3.org/2001/XMLSchema#nonNegativeInteger">1</owl:qualifiedCardinality>
                <owl:onClass rdf:resource="https://github.com/DeperiasKerre/qcl_Onto/blob/main/qclontology/qclontov1.owl#LaserDesignType"/>
            </owl:Restriction>
        </rdfs:subClassOf>
         <rdfs:label xml:lang="en">Heterostructure</rdfs:label>
         <rdfs:comment xml:lang="en">A layered material composed of different semiconductor materials.</rdfs:comment>
    </owl:Class>

    <!--LaserWorkingMode-->

    <owl:Class rdf:about="https://github.com/DeperiasKerre/qcl_Onto/blob/main/qclontology/qclontov1.owl#LaserWorkingMode">
         <rdfs:label xml:lang="en">Laser Working Mode</rdfs:label>
         <rdfs:comment xml:lang="en">This refers to the nature in which the laser beam is emitted.</rdfs:comment>
    </owl:Class>

    <!--PhysicalProperty-->

    <owl:Class rdf:about="https://w3id.org/mdo/core/PhysicalProperty">
        <rdfs:subClassOf rdf:resource="https://w3id.org/mdo/core/Property"/>
        <rdfs:subClassOf>
            <owl:Restriction>
                <owl:onProperty rdf:resource="https://github.com/DeperiasKerre/qcl_Onto/blob/main/qclontology/qclontov1.owl#correspondsToWorkingMode"/>
                <owl:qualifiedCardinality rdf:datatype="http://www.w3.org/2001/XMLSchema#nonNegativeInteger">1</owl:qualifiedCardinality>
                <owl:onClass rdf:resource="https://github.com/DeperiasKerre/qcl_Onto/blob/main/qclontology/qclontov1.owl#LaserWorkingMode"/>
            </owl:Restriction>
        </rdfs:subClassOf>
        <rdfs:comment xml:lang="en">A physical property is an objective property over a physical system. (ie, a property pertains to the physical reality)</rdfs:comment>
        <rdfs:label xml:lang="en">Physical Property</rdfs:label>
    </owl:Class>

    <!--Property-->

    <owl:Class rdf:about="https://w3id.org/mdo/core/Property">
        <rdfs:subClassOf rdf:resource="http://qudt.org/schema/qudt/Quantity"/>
        <rdfs:comment xml:lang="en">A property in materials design is data pertaining to at least one material or materials system.</rdfs:comment>
        <rdfs:label xml:lang="en">Property</rdfs:label>
    </owl:Class>

    <!--QuantityKind-->

    <owl:Class rdf:about="http://qudt.org/schema/qudt/QuantityKind">
        <rdfs:comment xml:lang="en">A Quantity Kind is any observable property that can be measured and quantified numerically.</rdfs:comment>
    </owl:Class>

    <!--Class Material-->

    <owl:Class rdf:about="http://emmo.info/domains/emmo-material.owl#EMMO_4207e895_8b83_4318_996a_72cfb32acd94">
        <rdfs:label xml:lang="en">Material</rdfs:label>
    </owl:Class>

    <!--LaserDesignType-->

    <owl:Class rdf:about="https://github.com/DeperiasKerre/qcl_Onto/blob/main/qclontology/qclontov1.owl#LaserDesignType">
         <rdfs:label xml:lang="en">Laser Design Type</rdfs:label>
         <rdfs:comment xml:lang="en">Ask Prof Kenneth.</rdfs:comment>
    </owl:Class>

    <!--MaterialComposition-->

    <owl:Class rdf:about="https://github.com/DeperiasKerre/qcl_Onto/blob/main/qclontology/qclontov1.owl#MaterialComposition">
         <rdfs:label xml:lang="en">Material Composition</rdfs:label>
         <rdfs:comment xml:lang="en">The refers to the different semiconductor materials forming the the heterostructure layer, including the combination ratio.</rdfs:comment>
    </owl:Class>

    <!--QuantityValue -->

    <owl:Class rdf:about="http://qudt.org/schema/qudt/QuantityValue">
         <rdfs:comment xml:lang="en">A Quantity Value expresses the magnitude and kind of a quantity.</rdfs:comment>
    </owl:Class>

    <!--Unit -->

    <owl:Class rdf:about="http://qudt.org/schema/qudt/Unit">

    <rdfs:comment xml:lang="en">A unit of measure, or unit, is a particular quantity value that has been chosen as a scale for measuring other quantities the same kind (more generally of equivalent dimension).</rdfs:comment>
    </owl:Class>

    <!--prov#Agent -->

    <owl:Class rdf:about="http://www.w3.org/ns/prov#Agent">
         <rdfs:subClassOf rdf:resource="http://www.w3.org/2002/07/owl#Thing"/>
         <rdfs:comment xml:lang="en">An agent is something that bears some form of responsibility for an activity taking place, for the existence of an entity, or for another agent's activity.</rdfs:comment>
    </owl:Class>

    <!--ReferenceInfoAgent-->

     <owl:Class rdf:about="https://github.com/DeperiasKerre/qcl_Onto/blob/main/qclontology/qclontov1.owl#ReferenceInfoAgent">
         <rdfs:subClassOf rdf:resource="http://www.w3.org/ns/prov#Agent"/>
         <rdfs:label xml:lang="en">ReferenceInfoAgent</rdfs:label>
         <rdfs:comment xml:lang="en">A ReferenceInnfoAgent is a scientific article documenting the laser design and properties</rdfs:comment>
    </owl:Class>

</rdf:RDF>